decoupling discussion and start of safe example

Coq/expose.v
@@ -1,125 +1,237 @@
 Require Import common.
 Require Import loo_def.
 Require Import chainmail.
-Require Import fundamental_properties.
+Require Import loo_properties.
+Require Import loo_reduction_properties.
 Require Import classical_properties.
-Require Import rename_equality.
+Require Import chainmail_extended_properties.
+Require Import function_operations.
 Require Import List.
 Require Import CpdtTactics.
 Require Import Coq.Logic.FunctionalExtensionality.
 
-(** #<h3># Expose example: #</h3># *)
-(** ---------------------------------------------------- *)
-(** #<code># >MyModule = { #</code># *)
-(** #<code># >  Inside = {} #</code># *)
-(** #<code># >  Boundary = { #</code># *)
-(** #<code># >    field inside : Inside #</code># *)
-(** #<code># >    meth expose() = {return this.inside} #</code># *)
-(** #<code># >  } #</code># *)
-(** #<code># >} #</code># *)
-(** --------------------------------------------------- *)
-(** #<code># we want to prove: #</code># *)
-(**  *)
-(** #<code># >MyModule ⊨  #</code># *)
-(** #<code># >(∀ b, b : Boundary, ∀ i, (b.inside = i ∧ (∀ x, x access i ⇒ x = b)) #</code># *)
-(** #<code># >             ⇒ (∀ p, will⟨ p access i ⟩ #</code># *)
-(** #<code># >               ⇒ (∃ o, will⟨ o calls b.expose() ⟩))) #</code># *)
-(**  *)
-(**  *)
+Module ExposeExample.
 
-Definition InsideID := classID 6.
+  (** #<h3># Safe example: #</h3># *)
+  (** ---------------------------------------------------- *)
+  (** #<code># >MyModule = { #</code># *)
+  (** #<code># >  Inside = {} #</code># *)
+  (** #<code># >  Boundary = { #</code># *)
+  (** #<code># >    field inside : Inside #</code># *)
+  (** #<code># >    meth expose() = {return this.inside} #</code># *)
+  (** #<code># >  } #</code># *)
+  (** #<code># >} #</code># *)
+  (** --------------------------------------------------- *)
+  (** #<code># we want to prove: #</code># *)
+  (**  *)
+  (** #<code># >MyModule ⊨  #</code># *)
+  (** #<code># >(∀ b, b : Boundary, ∀ i, (b.inside = i ∧ (∀ x, x access i ⇒ x = b)) #</code># *)
+  (** #<code># >             ⇒ (∀ p, will⟨ p access i ⟩ #</code># *)
+  (** #<code># >               ⇒ (∃ o, will⟨ o calls b.expose() ⟩))) #</code># *)
+  (**  *)
+  (**  *)
 
-Definition Boundary := classID 7.
+  (** Inside Definition  *)
 
-Definition InsideDef := clazz InsideID
-                              nil
-                              empty
-                              empty.
+  Definition Inside := classID 6.
 
-Definition inside := fieldID 0.
-
-Definition expose := methID 0.
-
-Definition x := bnd 10.
-
-Definition exposeBody := s_stmts (s_asgn (r_var x) (r_fld this inside))
-                                 (s_rtrn x).
-
-Definition BoundaryDef := clazz Boundary
-                                (inside :: nil)
-                                (update
-                                   expose (nil, exposeBody)
-                                   empty)
+  Definition InsideDef := clazz Inside
+                                nil
+                                empty
                                 empty.
 
-Definition MyModule := (update
-                          Boundary BoundaryDef
-                          (update
-                             InsideID InsideDef
-                             empty)).
+  (** Boundary Definition *)
 
-Ltac sat_destruct :=
-  match goal with
-  | [Hand : _ ⦂ _ ◎ _ ⊨ (_ ∧ _) |- _] => apply and_iff in Hand;
-                                       destruct Hand
-  end.
+  Definition Boundary := classID 7.
 
-Ltac frsh_auto :=
-  match goal with
-  | [Hfrsh : fresh_x _ _ (_ ∧ _) |- _] => apply fresh_and_elim in Hfrsh; andDestruct
-  | [Hfrsh : fresh_x _ _ (_ ⇒ _) |- _] => apply fresh_arr_elim in Hfrsh; andDestruct
-  | [Hfrsh : fresh_x _ _ (∀x∙ _) |- _] => apply fresh_all_elim in Hfrsh
-  | [ |- fresh_x _ _ (_ ∧ _)] => apply fresh_and_intro
-  | [ |- fresh_x _ _ (_ ⇒ _)] => apply fresh_arr_intro
-  | [ |- fresh_x _ _ (∀x∙_)] => apply fresh_all_intro
-  | [ Hfrsh : fresh_x ?x ?σ _ |- fresh_x ?x ?σ _] => auto; try (eapply fresh_notin; eauto)
-  end.
+  Definition inside := fieldID 0.
 
-Ltac a_intro :=
-  match goal with
-  | [|- _ ⦂ _ ◎ _ ⊨ (∀x∙ _)] => apply sat_all_x; intros; simpl
-  | [|- _ ⦂ _ ◎ _ ⊨ (_ ⇒ _)] => apply arr_prop1; intros; simpl
-  end.
+  Definition expose := methID 0.
 
-Ltac a_intros :=
-  repeat a_intro.
+  Definition x := bnd 10.
 
-Ltac a_prop :=
-  repeat match goal with
-         | [H : _ ⦂ _ ◎ _ ⊨ (_ ∧ _) |- _] => apply -> and_iff in H;
-                                           destruct H
-         | [H : _ ⦂ _ ◎ _ ⊨ (_ ∧ _) |- _] => apply -> or_iff in H
-         | [H : _ ⦂ _ ◎ _ ⊨ (_ ⇒ _) |- _] => rewrite -> arr_prop in H
-         | [H : context[_ ⦂ _ ◎ _ ⊨ (_ ⇒ _)] |- _] => rewrite -> arr_prop in H
-         | [H : _ ⦂ _ ◎ _ ⊨ (∀x∙_) |- _] => rewrite all_x_prop in H; simpl in H
-         | [|- _ ⦂ _ ◎ _ ⊨ (_ ∧ _)] => apply sat_and
-         | [|- _ ⦂ _ ◎ _ ⊨ (_ ∨ _)] => apply <- or_iff
-         end.
+  Definition exposeBody := s_stmts (s_asgn (r_var x) (r_fld this inside))
+                                   (s_rtrn x).
 
-Lemma expose_example :
-  entails (∀x∙∀x∙
-            ((a_class (e_hole 1) Boundary)
-             ∧
-             (a_eq (e_acc_f (e_hole 1) inside) (e_hole 0)))
-            ∧
-            (∀x∙((a_hole 0) access (a_hole 1) ⇒ (a_eq (e_hole 0) (e_hole 2)))))
-          (∀x∙∀x∙
-            ((a_class (e_hole 1) Boundary)
-             ∧
-             (a_eq (e_acc_f (e_hole 1) inside) (e_hole 0)))
-            ∧(¬ ∃x∙(((a_hole 0) access (a_hole 1)) ∧ ¬(a_class (e_hole 0) Boundary)))).
-Proof.
-  auto.
-  apply ent;
-    intros.
-  a_intros.
-  repeat (a_prop;
-          a_intros;
-          auto).
+  Definition BoundaryDef := clazz Boundary
+                                  (inside :: nil)
+                                  (update
+                                     expose (nil, exposeBody)
+                                     empty)
+                                  empty.
 
-  - unfold mapp, configMapStack in *;
+  (** MyModule Definition *)
+
+  Definition MyModule := (update
+                            Boundary BoundaryDef
+                            (update
+                               Inside InsideDef
+                               empty)).
+
+
+  Theorem expose_example_will :
+    MyModule ⊨m (∀x∙∀x∙(((a_class (e♢1) Boundary)
+                         ∧
+                         ((e_acc_f (e♢1) inside) ⩦ (e♢0))
+                         ∧
+                         ((guards (a♢1) (a♢0))))
+                        ∧
+                        (a_will (¬ guards (a♢1) (a♢0)))
+                          ⇒
+                          (a_will (∃x∙((a♢0) calls (a♢2) ∎ expose ⟨ empty ⟩)) ∨
+                           ((a_ this) calls (a♢1) ∎ expose ⟨ empty ⟩)))).
+  Proof.
+    unfold mdl_sat;
+      intros;    
+      repeat (a_intros; a_prop);
       simpl in *.
-    unfold mapp in *.
-    apply sat_class with (α:=).
+    
+    repeat destruct_exists_loo.
+    destruct σ as [χ]; simpl in *; subst.
 
-Qed.
+    inversion H6; subst.
+    inversion H10; subst.
+
+    - right.
+      admit.
+
+    - assert (σ_wf (χ0, ϕ0::ψ0)).
+      match goal with
+      | [H : update_σ_map _ _ _ = ?σ |- context[?σ]] =>
+        rewrite <- H
+      end.
+      repeat (eapply σ_wf_update; eauto).
+      apply arising_wf with (M1:=MyModule)(M2:=M'); auto.
+      let someσ := fresh "σ" in
+      destruct (adaptation_exists_wf (χ0,ϕ0::ψ0) σ) as [someσ];
+        auto.
+      apply pair_reduction_preserves_config_wf
+        with (M1:=MyModule)(M2:=M')
+             (σ1:=(χ0, ϕ0::nil));
+        auto.
+      eapply σ_wf_top_frame; eauto.
+
+      destruct (sat_excluded_middle MyModule M' σ0 (guards (a_ z) (a_ z0))) as [Hsat|Hnsat].
+
+      + destruct will_change_pair_reduction
+          with (M1:=MyModule)(M2:=M')
+               (A:=guards (a_ z) (a_ z0))
+               (σ1:=σ)(σ1':=σ0)
+               (σ2:=σ')(σ2':=σ'')
+               (σ:=(χ0,ϕ0::ψ0));
+          eauto with loo_db.
+        * crush.
+        * repeat destruct_exists_loo;
+            andDestruct.
+          left.
+          let Ha := fresh "H" in
+          let Hb := fresh "H" in
+          destruct (pair_reductions_alt_definition MyModule M' σ σ1)
+            as [Ha Hb];
+            match goal with
+            | [H : MyModule ⦂ M' ⦿ σ ⤳⋆ σ1 |- _] =>
+              specialize (Ha H);
+                destruct Ha
+            end.
+
+          ** destruct (pair_reduction_change_implies_method_call MyModule M' σ σ1);
+               eauto with loo_db.
+             *** repeat destruct_exists_loo;
+                   andDestruct;
+                   subst.
+                 apply sat_will with (χ:=χ0)(ψ:=ψ0)(ϕ:=ϕ0)(σ':=(χ1,ϕ1::ψ1))(σ'':=σ0);
+                   eauto with loo_db.
+                 rewrite H9; auto.
+                 admit.
+
+             *** admit.
+
+          ** admit.
+
+        * admit.
+
+      + admit.
+
+  Admitted.
+
+  (**
+     expose_example_was does not work, because there is no way to ensure that 
+     some frame in the stack below the identified frame in the past does not
+     have access to inside. Thus, access could be granted purely by returning 
+     from some method call. expose_example_will works because will restricts
+     the stack to just the top frame, thus removing the possibility of returning
+     to some lower frame.
+   *)
+
+  Theorem expose_example_was :
+    MyModule ⊨m (∀x∙∀x∙((a_was (((a_class (e♢1) Boundary)
+                                 ∧
+                                 ((e_acc_f (e♢1) inside) ⩦ (e♢0)))
+                                ∧
+                                ((guards (a♢1) (a♢0))))
+                         ∧
+                         (¬ guards (a♢1) (a♢0)))
+                          ⇒
+                          a_was(∃x∙((a♢0) calls (a♢2) ∎ expose ⟨ empty ⟩)))).
+  Proof.
+    unfold mdl_sat;
+      intros.
+    repeat (a_intros; a_prop).
+    simpl in *.    
+
+    inversion H5; subst.
+    apply sat_was; intros.
+    specialize (H11 σ0);
+      repeat auto_specialize.
+    destruct H11 as [σ' Htmp];
+      destruct Htmp as [σ''];
+      andDestruct.
+    inversion Hb; subst.
+
+    assert (Hwf : σ_wf σ');
+      [eauto with loo_db|].
+
+    destruct (was_change_pair_reduction MyModule M')
+      with (σ:=(update_σ_map (update_σ_map σ z v) z0 v0))
+           (σ':=σ')(A:=¬ guards (a_ z) (a_ z0))(σ'':=σ'')
+      as [Hwas|Hwas];
+      auto;
+      [apply sat_not, nsat_not; auto| |destruct Hwas as [Hwas|Hwas]].
+
+    - destruct Hwas as [σ1 Htmp];
+        destruct Htmp as [σ1' Htmp];
+        destruct Htmp as [σ2 Htmp];
+        destruct Htmp as [σ2' Htmp];
+        andDestruct.
+      exists σ1, σ1';
+        repeat split; eauto with loo_db.
+      destruct (pair_reduction_change_implies_method_call MyModule M' σ1 σ2)
+        as [Hcont|Hcont];
+        eauto with loo_db;
+        [|destruct Hcont as [Hcont|Hcont]].
+      * destruct Hcont as [χ1 Hcont];
+          destruct Hcont as [ϕ1 Hcont];
+          destruct Hcont as [ψ1 Hcont];
+          destruct Hcont as [x' Hcont];
+          destruct Hcont as [y' Hcont];
+          destruct Hcont as [m Hcont];
+          destruct Hcont as [ps Hcont];
+          destruct Hcont as [s Hcont];
+          andDestruct;
+          subst.
+
+        admit.
+
+      * admit.
+
+      * admit.
+
+    - destruct Hwas as [σ1 Htmp];
+        destruct Htmp as [σ1' Htmp];
+        andDestruct.
+      exists σ1, σ1';
+        repeat split; eauto with loo_db.
+    
+  Abort.
+
+End ExposeExample.
