Coq/chainmail_extended_properties.v
@@ -1,0 +1,1721 @@
+Require Import common.
+Require Import loo_def.
+Require Import chainmail.
+Require Import loo_properties.
+Require Import loo_reduction_properties.
+Require Import function_operations.
+Require Import sbst.
+Require Import classical_properties.
+Require Import List.
+Require Import String.
+Open Scope string_scope.
+Require Import CpdtTactics.
+Require Import Coq.Logic.FunctionalExtensionality.
+
+Lemma prev_neg :
+  forall M1 M2 σ A, M1 ⦂ M2 ◎ σ ⊨ (¬ a_prev A) ->
+               (exists σ0 σ' σ'', initial σ0 ->
+                             M1 ⦂ M2 ⦿ σ0 ⤳⋆ σ' ->
+                             M1 ⦂ M2 ⦿ σ' ⤳ σ ->
+                             σ ◁ σ' ≜ σ'' ->
+                             M1 ⦂ M2 ◎ σ'' ⊨ (¬ A)).
+Proof.
+  intros.
+Admitted.
+
+Lemma was_neg :
+  forall M1 M2 σ A, M1 ⦂ M2 ◎ σ ⊨ (¬ a_was A) ->
+               (exists σ0 σ' σ'', initial σ0 ->
+                             M1 ⦂ M2 ⦿ σ0 ⤳⋆ σ' ->
+                             M1 ⦂ M2 ⦿ σ' ⤳⋆ σ ->
+                             σ ◁ σ' ≜ σ'' ->
+                             M1 ⦂ M2 ◎ σ'' ⊨ (¬ A)).
+Proof.
+Admitted.
+
+Lemma prev_not_disj :
+  forall A1 A2, entails (a_prev (A1 ∨ A2) ∧ (a_prev (¬ A1)))
+                   (a_prev A2).
+Proof.
+  intros;
+    apply ent;
+    intros;
+    a_prop.
+
+  inversion H; subst.
+  apply sat_prev; intros.
+  specialize (H5 σ0 σ' σ'' H1 H2 H3 H4);
+    a_prop.
+  destruct H5; auto.
+  inversion H0; subst.
+  specialize (H10 σ0 σ' σ'' H1 H2 H3 H4);
+    a_prop.
+Qed.
+
+Lemma prev_disj :
+  forall A1 A2, entails ((a_prev A1) ∨ (a_prev A2))
+                   (a_prev (A1 ∨ A2)).
+Proof.
+  intros.
+  apply ent;
+    intros.
+  a_prop.
+  destruct H.
+  - apply sat_prev; intros.
+    inversion H; subst.
+    specialize (H8 σ0 σ' σ'' H0 H1 H2 H3);
+      a_prop; auto.
+  - apply sat_prev; intros.
+    inversion H; subst.
+    specialize (H8 σ0 σ' σ'' H0 H1 H2 H3);
+      a_prop; auto.
+Qed.
+
+Hint Resolve prev_disj : chainmail_db.
+
+Lemma will_was_1 :
+  forall A, entails (a_will (a_was A))
+               ((a_was A) ∨ A ∨ (a_will A)).
+Proof.
+Admitted. (* is this even true? future is deterministic, past is non-deterministic *)
+
+Lemma will_was_2 :
+  forall A, entails ((a_was A) ∨ A ∨ (a_will A))
+               (a_will (a_was A)).
+Proof.
+Admitted.
+
+Lemma was_will :
+  forall A, entails (a_was (a_will A))
+               (a_will (a_was A)).
+Proof.
+  intros.
+  apply ent;
+    intros.
+  
+Admitted.
+
+Lemma was_change_pair_reduction :
+  forall M1 M2 σ' σ, M1 ⦂ M2 ⦿ σ' ⤳⋆ σ ->
+                σ_wf σ' ->
+                forall A, M1 ⦂ M2 ◎ σ ⊨ A ->
+                     forall σ'', σ ◁ σ' ≜ σ'' ->
+                            M1 ⦂ M2 ◎ σ'' ⊨ (¬ A) ->
+                            (exists σ1 σ1' σ2 σ2', M1 ⦂ M2 ⦿ σ' ⤳⋆ σ1 /\
+                                              M1 ⦂ M2 ⦿ σ1 ⤳ σ2 /\
+                                              M1 ⦂ M2 ⦿ σ2 ⤳⋆ σ /\
+                                              σ ◁ σ1 ≜ σ1' /\
+                                              σ ◁ σ2 ≜ σ2' /\
+                                              M1 ⦂ M2 ◎ σ1' ⊨ (¬ A) /\
+                                              M1 ⦂ M2 ◎ σ2' ⊨ A) \/
+                            (exists σa σb, M1 ⦂ M2 ⦿ σ' ⤳⋆ σa /\
+                                      M1 ⦂ M2 ⦿ σa ⤳ σ /\
+                                      σ ◁ σa ≜ σb /\
+                                      M1 ⦂ M2 ◎ σb ⊨ (¬ A)) \/
+                            (exists σa σb, M1 ⦂ M2 ⦿ σ' ⤳ σa /\
+                                      M1 ⦂ M2 ⦿ σa ⤳⋆ σ /\
+                                      σ ◁ σa ≜ σb /\
+                                      M1 ⦂ M2 ◎ σb ⊨ A) \/
+                            (M1 ⦂ M2 ⦿ σ' ⤳ σ).
+Proof.
+  intros M1 M2 σ' σ Hred;
+    induction Hred;
+    intros;
+    auto.
+
+  - specialize (IHHred (pair_reduction_preserves_config_wf M1 M2 σ1 σ H H0) A H1).
+    let someσ := fresh "σ" in
+    destruct (adaptation_exists_wf σ2 σ) as [someσ];
+      eauto with loo_db.
+    destruct (sat_excluded_middle M1 M2 σ0 A).
+    + right; right; left.
+      eexists; eauto with loo_db.
+    + apply sat_not in H5.
+      specialize (IHHred σ0 H4 H5).
+      destruct IHHred as [IH|IH];
+        [|destruct IH as [IH|IH];
+          [|destruct IH as [IH|IH]]].
+      * let someσ1 := fresh "σ" in
+         let someσ2 := fresh "σ" in
+         let someσ3 := fresh "σ" in
+         let someσ4 := fresh "σ" in
+         destruct IH as [someσ1 Htmp];
+           destruct Htmp as [someσ2 Htmp];
+           destruct Htmp as [someσ3 Htmp];
+           destruct Htmp as [someσ4];
+           andDestruct;
+           left;
+           exists someσ1, someσ2, someσ3, someσ4;
+           repeat split; eauto with loo_db.
+      * let someσ1 := fresh "σ" in
+         let someσ2 := fresh "σ" in
+         destruct IH as [someσ1 Htmp];
+           destruct Htmp as [someσ2 Htmp];
+           andDestruct;
+           right;
+           left;
+           exists σ3, σ4;
+           repeat split; eauto with loo_db.
+      * let someσ1 := fresh "σ" in
+         let someσ2 := fresh "σ" in
+         destruct IH as [someσ1 Htmp];
+           destruct Htmp as [someσ2 Htmp];
+           andDestruct;
+           left;
+           exists σ, σ0, someσ1, someσ2;
+           repeat split; eauto with loo_db.
+      * right; left;
+          exists σ, σ0;
+          eauto with loo_db.
+Qed.
+
+Inductive pair_reductions_alt : mdl -> mdl -> config -> config -> Prop :=
+| prs_single' : forall M1 M2 σ1 σ2, M1 ⦂ M2 ⦿ σ1 ⤳ σ2 ->
+                               pair_reductions_alt M1 M2 σ1 σ2
+| prs_trans'  : forall M1 M2 σ1 σ σ2, pair_reductions_alt M1 M2 σ1 σ ->
+                                 M1 ⦂ M2 ⦿ σ ⤳ σ2 ->
+                                 pair_reductions_alt M1 M2 σ1 σ2.
+
+Hint Constructors pair_reductions_alt : loo_db.
+
+Lemma pair_reductions_alt_implies_pair_reductions :
+  forall M1 M2 σ1 σ2, pair_reductions_alt M1 M2 σ1 σ2 ->
+                 M1 ⦂ M2 ⦿ σ1 ⤳⋆ σ2.
+Proof.
+  intros M1 M2 σ1 σ2 Hred;
+    induction Hred;
+    eauto with loo_db.
+  apply pair_reductions_transitive with (σ2:=σ); auto with loo_db.
+Qed.
+
+Hint Resolve pair_reductions_alt_implies_pair_reductions : loo_db.
+Hint Rewrite pair_reductions_alt_implies_pair_reductions : loo_db.
+
+Lemma pair_reductions_alt_extend :
+  forall M1 M2 σ1 σ2, pair_reductions_alt M1 M2 σ1 σ2 ->
+                 forall σ, M1 ⦂ M2 ⦿ σ ⤳ σ1 ->
+                      pair_reductions_alt M1 M2 σ σ2.
+Proof.
+  intros M1 M2 σ1 σ2 Hred;
+    induction Hred;
+    intros;
+    eauto with loo_db.
+Qed.
+
+Lemma pair_reductions_implies_pair_reductions_alt :
+  forall M1 M2 σ1 σ2, M1 ⦂ M2 ⦿ σ1 ⤳⋆ σ2 ->
+                 pair_reductions_alt M1 M2 σ1 σ2.
+Proof.
+  intros M1 M2 σ1 σ2 Hred;
+    induction Hred;
+    eauto with loo_db.
+  apply pair_reductions_alt_extend with (σ1:=σ); auto with loo_db.
+Qed.
+
+Hint Resolve pair_reductions_implies_pair_reductions_alt : loo_db.
+Hint Rewrite pair_reductions_implies_pair_reductions_alt : loo_db.
+
+Lemma pair_reductions_alt_definition :
+  forall M1 M2 σ1 σ2, M1 ⦂ M2 ⦿ σ1 ⤳⋆ σ2 <->
+                 (M1 ⦂ M2 ⦿ σ1 ⤳ σ2) \/
+                 (exists σ, M1 ⦂ M2 ⦿ σ1 ⤳⋆ σ /\
+                       M1 ⦂ M2 ⦿ σ ⤳⋆ σ2).
+Proof.
+  intros M1 M2 σ1 σ2;
+    split;
+    [intro Hred;
+     induction Hred;
+     eauto with loo_db
+    |intro Hred;
+     destruct Hred;
+     eauto with loo_db].
+
+  - repeat destruct_exists_loo;
+      andDestruct;
+      eauto with loo_db.
+    eapply pair_reductions_transitive; eauto.
+
+Qed.
+
+Inductive reductions : mdl -> config -> config -> Prop :=
+| red_single : forall M σ1 σ2, M ∙ σ1 ⤳ σ2 ->
+                          reductions M σ1 σ2
+| red_trans : forall M σ1 σ2 σ3, reductions M σ1 σ2 ->
+                            M ∙ σ2 ⤳ σ3 ->
+                            reductions M σ1 σ3.
+
+Hint Constructors reductions : loo_db.
+
+Lemma list_does_not_contain_itself :
+  forall {A : Type} (l : list A) a,
+    a :: l = l ->
+    False.
+Proof.
+  intros A l;
+    induction l;
+    intros;
+    crush.
+Qed.
+
+Inductive substmt : stmt -> stmt -> Prop :=
+| sub_eq1 : forall s s', substmt s (s_stmts s s')
+| sub_eq2 : forall s s', substmt s (s_stmts s' s)
+| sub_trns1 : forall s s1 s2, substmt s s1 ->
+                         substmt s (s_stmts s1 s2)
+| sub_trns2 : forall s s1 s2, substmt s s2 ->
+                         substmt s (s_stmts s1 s2).
+
+Hint Constructors substmt : loo_db.
+
+Parameter stmt_not_strict_substatement_of_itself :
+  forall s s', substmt s s' ->
+          s = s' ->
+          False.
+
+Lemma acyclic_reduction :
+  forall M σ1 σ2, M ∙ σ1 ⤳ σ2 ->
+             σ2 <> σ1.
+Proof.
+  intros M σ1 σ2 Hred;
+    induction Hred;
+    intro Hcontra;
+    subst.
+
+  - match goal with
+    | [H : (_, _) = (_, _) |- _] =>
+      inversion H; subst;
+        simpl in *
+    end.
+    apply list_does_not_contain_itself in H8; auto.
+
+  - match goal with
+    | [H : (_, _) = (_, _) |- _] =>
+      inversion H; subst;
+        simpl in *
+    end.
+    rewrite <- H7 in H1;
+      simpl in *.
+    inversion H1; subst.
+    eapply stmt_not_strict_substatement_of_itself;
+      eauto with loo_db.
+
+  - match goal with
+    | [H : (_, _) = (_, _) |- _] =>
+      inversion H; subst;
+        simpl in *
+    end.
+    rewrite <- H8 in H0;
+      simpl in *.
+    inversion H0; subst.
+    eapply stmt_not_strict_substatement_of_itself;
+      eauto with loo_db.
+
+  - match goal with
+    | [H : (_, _) = (_, _) |- _] =>
+      inversion H; subst;
+        simpl in *
+    end.
+    rewrite <- H7 in H1;
+      simpl in *.
+    inversion H1; subst.
+    eapply stmt_not_strict_substatement_of_itself;
+      eauto with loo_db.
+
+  - match goal with
+    | [H : (_, _) = (_, _) |- _] =>
+      inversion H; subst;
+        simpl in *
+    end.
+    eapply list_does_not_contain_itself; eauto.
+
+  - match goal with
+    | [H : (_, _) = (_, _) |- _] =>
+      inversion H; subst;
+        simpl in *
+    end.
+    eapply list_does_not_contain_itself; eauto.
+Qed.
+
+Hint Resolve acyclic_reduction : loo_db.
+
+Lemma acyclic_reductions :
+  forall M σ1 σ2, reductions M σ1 σ2 ->
+             σ2 <> σ1.
+Proof.
+  intros M σ1 σ2 Hred;
+    induction Hred.
+
+  - eauto with loo_db.
+
+  - intro Hcontra;
+      subst.
+  
+Admitted.
+
+Lemma acyclic_pair_reductions :
+  forall M1 M2 σ1 σ2, M1 ⦂ M2 ⦿ σ1 ⤳⋆ σ2 ->
+                 σ1 <> σ2.
+Proof.
+Admitted.
+
+Lemma pair_reductions_path_unique :
+  forall M1 M2 σ1 σ2, M1 ⦂ M2 ⦿ σ1 ⤳ σ2 ->
+                 forall σ, M1 ⦂ M2 ⦿ σ1 ⤳⋆ σ ->
+                      M1 ⦂ M2 ⦿ σ ⤳⋆ σ2 ->
+                      False.
+Proof.
+Admitted.
+
+Lemma adaptation_satisfaction :
+  forall M1 M2 σ A, M1 ⦂ M2 ◎ σ ⊨ A ->
+               forall σ1 σ2 σ', σ1 ◁ σ2 ≜ σ ->
+                           σ1 ◁ σ2 ≜ σ' ->
+                           M1 ⦂ M2 ◎ σ' ⊨ A.
+Proof.
+Admitted.
+
+Lemma will_change_pair_reduction :
+  forall M1 M2 σ1 σ2, M1 ⦂ M2 ⦿ σ1 ⤳⋆ σ2 ->
+                 forall σ, σ_wf σ ->
+                      σ_wf σ1 ->
+                      forall σ1' σ2', σ ◁ σ1 ≜ σ1' ->
+                                 σ ◁ σ2 ≜ σ2' ->
+                                 forall A, M1 ⦂ M2 ◎ σ1' ⊨ A ->
+                                      M1 ⦂ M2 ◎ σ2' ⊨ (¬ A) ->
+                                      (exists σa σb, M1 ⦂ M2 ⦿ σ1 ⤳⋆ σa /\
+                                                σ ◁ σa ≜ σb /\
+                                                M1 ⦂ M2 ◎ σb ⊨ (¬ A) /\
+                                                (forall σa' σb', M1 ⦂ M2 ⦿ σ1 ⤳⋆ σa' ->
+                                                            M1 ⦂ M2 ⦿ σa' ⤳⋆ σa ->
+                                                            σ ◁ σa' ≜ σb' ->
+                                                            M1 ⦂ M2 ◎ σb' ⊨ A)) \/
+                                      (M1 ⦂ M2 ⦿ σ1 ⤳ σ2).
+Proof.
+  intros M1 M2 σ1 σ2 Hred;
+    induction Hred;
+    intros;
+    eauto with loo_db.
+
+  - assert (Hwf : σ_wf σ);
+      [eauto with loo_db|].
+    let someσ := fresh "σ" in
+    let Hadapt := fresh "H" in
+    destruct (adaptation_exists_wf σ0 σ) as [someσ Hadapt];
+      auto;
+      destruct (sat_excluded_middle M1 M2 σ3 A) as [Hsat|Hnsat];
+      specialize (IHHred σ0);
+      repeat auto_specialize;
+      specialize (IHHred someσ σ2');
+      repeat auto_specialize.
+
+    + specialize (IHHred A);
+        repeat auto_specialize.
+      destruct IHHred as [IH|IH].
+
+      * repeat destruct_exists_loo;
+          andDestruct.
+        left.
+        exists σ4, σ5;
+          repeat split;
+          eauto with loo_db;
+          intros.
+        specialize (Hb σa' σb').
+        inversion H7; subst.
+        ** apply pair_reduction_unique with (σ2:=σ) in H10;
+             auto;
+             subst.
+           eapply adaptation_satisfaction; eauto.
+        ** apply pair_reduction_unique with (σ2:=σ) in H10;
+             auto;
+             subst.
+           apply Hb; auto.
+
+      * left.
+        exists σ2, σ2';
+          repeat split;
+          eauto with loo_db;
+          intros.
+        inversion H7; inversion H8; subst.
+        ** apply pair_reduction_unique with (σ2:=σ) in H10;
+             auto;
+             subst.
+           eapply adaptation_satisfaction; eauto.
+        ** apply pair_reduction_unique with (σ2:=σ) in H10;
+             auto;
+             subst.
+           apply pair_reduction_unique with (σ2:=σ2) in H15;
+             auto;
+             subst.
+           eapply adaptation_satisfaction; eauto.
+        ** apply pair_reduction_unique with (σ2:=σ) in H10;
+             auto;
+             subst.
+           apply pair_reductions_path_unique with (σ:=σa') in IH;
+             crush.
+        ** apply pair_reduction_unique with (σ2:=σ) in H10;
+             auto;
+             subst.
+           apply pair_reductions_path_unique with (σ:=σa') in IH;
+             crush.
+
+    + left; exists σ, σ3;
+        repeat split;
+        eauto with loo_db;
+        [apply sat_not; auto|intros].
+      apply pair_reductions_path_unique with (σ:=σa') in H;
+        crush.
+Qed.
+
+(*Lemma will_change_pair_reduction :
+  forall M1 M2 σ σ', pair_reductions_alt M1 M2 σ σ' ->
+                σ_wf σ ->
+                forall A, M1 ⦂ M2 ◎ σ ⊨ A ->
+                     forall σ'', σ ◁ σ' ≜ σ'' ->
+                            M1 ⦂ M2 ◎ σ'' ⊨ (¬ A) ->
+                            (forall σa' σb', pair_reductions_alt M1 M2 σ σa' /\
+                                        pair_reductions_alt M1 M2 σa' σ' /\
+                                        σ ◁ σa' ≜ σb' /\
+                                        M1 ⦂ M2 ◎ σb' ⊨ A) \/
+                            (exists σa σb, pair_reductions_alt M1 M2 σ σa /\
+                                      σ ◁ σa ≜ σb /\
+                                      M1 ⦂ M2 ◎ σb ⊨ (¬ A) /\
+                                      (forall σa' σb', pair_reductions_alt M1 M2 σ σa' /\
+                                                  pair_reductions_alt M1 M2 σa' σa /\
+                                                  σ ◁ σa' ≜ σb' /\
+                                                  M1 ⦂ M2 ◎ σb' ⊨ A)) \/
+                            (exists σa σb, M1 ⦂ M2 ⦿ σ ⤳ σa /\
+                                      σ ◁ σa ≜ σb /\
+                                      M1 ⦂ M2 ◎ σb ⊨ (¬ A)).
+Proof.
+  intros M1 M2 σ σ' Hred;
+    induction Hred;
+    intros.
+
+  - right; right; eauto with loo_db.
+
+  - let someσ := fresh "σ" in
+    let Hadapt := fresh "H" in
+    destruct (exists_adaptation σ1 σ) as [someσ Hadapt];
+      eauto with loo_db;
+      specialize (IHHred H0 A H1 someσ Hadapt).
+    destruct (sat_excluded_middle M1 M2 σ0 A).
+    + 
+
+      
+    (pair_reduction_preserves_config_wf M1 M2 σ1 σ H H0) A H1).
+    let someσ := fresh "σ" in
+    destruct (exists_adaptation σ2 σ) as [someσ];
+      eauto with loo_db.
+    destruct (sat_excluded_middle M1 M2 σ0 A).
+    + right; right; left.
+      eexists; eauto with loo_db.
+    + apply sat_not in H5.
+      specialize (IHHred σ0 H4 H5).
+      destruct IHHred as [IH|IH];
+        [|destruct IH as [IH|IH];
+          [|destruct IH as [IH|IH]]].
+      * let someσ1 := fresh "σ" in
+         let someσ2 := fresh "σ" in
+         let someσ3 := fresh "σ" in
+         let someσ4 := fresh "σ" in
+         destruct IH as [someσ1 Htmp];
+           destruct Htmp as [someσ2 Htmp];
+           destruct Htmp as [someσ3 Htmp];
+           destruct Htmp as [someσ4];
+           andDestruct;
+           left;
+           exists someσ1, someσ2, someσ3, someσ4;
+           repeat split; eauto with loo_db.
+      * let someσ1 := fresh "σ" in
+         let someσ2 := fresh "σ" in
+         destruct IH as [someσ1 Htmp];
+           destruct Htmp as [someσ2 Htmp];
+           andDestruct;
+           right;
+           left;
+           exists σ3, σ4;
+           repeat split; eauto with loo_db.
+      * let someσ1 := fresh "σ" in
+         let someσ2 := fresh "σ" in
+         destruct IH as [someσ1 Htmp];
+           destruct Htmp as [someσ2 Htmp];
+           andDestruct;
+           left;
+           exists σ, σ0, someσ1, someσ2;
+           repeat split; eauto with loo_db.
+      * right; left;
+          exists σ, σ0;
+          eauto with loo_db.
+Qed.*)
+
+Lemma interpret_update :
+  forall x σ y v v', ⌊ x ⌋ (update_σ_map σ y v) ≜ v' ->
+                x <> y ->
+                ⌊ x ⌋ σ ≜ v'.
+Proof.
+  intros.
+  inversion H; subst.
+  destruct σ as [χ ψ'];
+    destruct ψ' as [|ϕ0 ψ0];
+    match goal with
+    | [H : _ = _ :: _ |- _] =>
+      inversion H; subst
+    end;
+    simpl in *;
+    subst.
+  unfold update, t_update in H2.
+  eq_auto.
+  eapply int_x;
+    simpl;
+    eauto with loo_db.
+Qed.
+
+Hint Resolve interpret_update : loo_db.
+
+Lemma class_of_update :
+  forall x σ y v C, classOf x (update_σ_map σ y v) C ->
+               x <> y ->
+               classOf x σ C.
+Proof.
+  intros.
+  inversion H; subst.
+  apply interpret_update in H1;
+    auto.
+  eapply cls_of;
+    eauto.
+Qed.
+
+Hint Resolve class_of_update : loo_db.
+
+Lemma interpret_update_vMap :
+  forall x χ ϕ ψ v, ⌊ x ⌋ (χ, ϕ::ψ) ≜ v ->
+               forall ϕ' y v', vMap ϕ = update y v' (vMap ϕ') ->
+                         x <> y ->
+                         ⌊ x ⌋ (χ, ϕ'::ψ) ≜ v.
+Proof.
+  intros.
+  inversion H; subst.
+  simpl in *;
+    match goal with
+    | [H : _ = _ :: _ |- _] =>
+      inversion H; subst
+    end;
+    simpl in *;
+    subst.
+  unfold update, t_update in H0.
+  apply equal_f with (x0:=x) in H0.
+  eq_auto.
+  eapply int_x;
+    simpl;
+    crush.
+Qed.
+
+Hint Resolve interpret_update_vMap : loo_db.
+
+Lemma class_of_update_vMap :
+  forall x χ ϕ ψ C, classOf x (χ, ϕ::ψ) C ->
+               forall ϕ' y v, vMap ϕ = update y v (vMap ϕ') ->
+                         x <> y ->
+                         classOf x (χ, ϕ'::ψ) C.
+Proof.
+  intros.
+  inversion H; subst.
+  apply interpret_update_vMap with (ϕ':=ϕ')(y:=y)(v':=v) in H2;
+    auto.
+  eapply cls_of;
+    eauto.
+Qed.
+
+Hint Resolve class_of_update_vMap : loo_db.
+
+Lemma class_of_unique :
+  forall x σ C C', classOf x σ C ->
+              classOf x σ C' ->
+              C' = C.
+Proof.
+  intros.
+  inversion H; subst.
+  inversion H0; subst.
+  interpretation_rewrite.
+  match goal with
+  | [H : v_addr ?α1 = v_addr ?α2,
+         Ha : ?f ?α1 = Some ?o1,
+         Hb : ?f ?α2 = Some ?o2 |- _] =>
+    inversion H;
+      subst;
+      rewrite Ha in Hb;
+      inversion Hb;
+      subst
+  end;
+    auto.
+Qed.
+
+Hint Resolve class_of_unique : loo_db.
+
+Lemma interpretation_same_variable_map :
+  forall x σ v, ⌊ x ⌋ σ ≜ v ->
+           forall χ ϕ ψ χ' ϕ' ψ',
+             σ = (χ, ϕ::ψ) ->
+             vMap ϕ' = vMap ϕ ->
+             ⌊ x ⌋ (χ', ϕ'::ψ') ≜ v.
+Proof.
+  intros;
+    subst.
+
+  inversion H; subst;
+    simpl in *.
+  match goal with
+  | [H : _::_ = _::_ |- _] =>
+    inversion H; subst
+  end.
+  eapply int_x;
+    simpl;
+    eauto with loo_db.
+  crush.
+Qed.
+
+Hint Resolve interpretation_same_variable_map : loo_db.
+Hint Rewrite interpretation_same_variable_map : loo_db.
+
+Lemma class_of_same_variable_map :
+  forall x σ C, classOf x σ C ->
+           forall χ ϕ ψ ϕ' ψ',
+             σ = (χ, ϕ::ψ) ->
+             vMap ϕ' = vMap ϕ ->
+             classOf x (χ, ϕ'::ψ') C.
+Proof.
+  intros;
+    subst.
+  inversion H; subst.
+  eapply cls_of;
+    eauto with loo_db.
+Qed.
+
+Hint Resolve interpretation_same_variable_map : loo_db.
+Hint Rewrite interpretation_same_variable_map : loo_db.
+
+Lemma interpret_x_update_heap_fresh :
+  forall x α vα χ ψ v, ⌊ x ⌋ (χ, ψ) ≜ v ->
+                  forall v', ⌊ x ⌋ (update α vα χ, ψ) ≜ v' ->
+                        fresh_χ χ α ->
+                        v' = v.
+Proof.
+  intros.
+  inversion H;
+    subst.
+  inversion H0;
+    subst.
+  simpl in *; subst.
+  crush.
+Qed.
+
+Hint Resolve interpret_x_update_heap_fresh : loo_db.
+Hint Rewrite interpret_x_update_heap_fresh : loo_db.
+
+Lemma class_of_update_heap_fresh :
+  forall x α v χ ψ C, classOf x (χ, ψ) C ->
+                 forall C', classOf x (update α v χ, ψ) C' ->
+                       fresh_χ χ α ->
+                       C' = C.
+Proof.
+  intros.
+  inversion H;
+    subst.
+  inversion H0;
+    subst.
+  simpl in *.
+  match goal with
+  | [Ha : ⌊ ?x ⌋ (?χ, ?ψ) ≜ ?v1,
+          Hb : ⌊ ?x ⌋ (?χ', ?ψ) ≜ ?v2 |- _] =>
+    eapply interpret_x_update_heap_fresh in Ha;
+      eauto;
+      inversion Ha;
+      subst
+  end.
+  destruct (eq_dec α α0);
+    subst;
+    repeat map_rewrite;
+    eq_auto.
+  - apply fresh_heap_none in H1; crush.
+  - crush.
+Qed.
+
+Hint Resolve class_of_update_heap_fresh : loo_db.
+Hint Rewrite class_of_update_heap_fresh : loo_db.
+
+Lemma class_of_update_same_cname :
+  forall x σ C, classOf x σ C ->
+           forall χ ψ, σ = (χ, ψ) ->
+                  forall α o o', χ α = Some o ->
+                            cname o' = cname o ->
+                            forall C', classOf x (update α o' χ, ψ) C' ->
+                                  C' = C.
+Proof.
+
+  Admitted.
+
+Lemma reduction_different_classes_implies_method_call_or_rtrn :
+  forall M σ1 σ2, M ∙ σ1 ⤳ σ2 ->
+             forall C1 C2, classOf this σ1 C1 ->
+                      classOf this σ2 C2 ->
+                      C1 <> C2 ->
+                      (exists χ1 ϕ1 ψ1 x0 y0 m ps s, σ1 = (χ1, ϕ1::ψ1) /\
+                                                contn ϕ1 = (c_stmt (s_stmts (s_meth x0 y0 m ps) s))) \/
+                      (exists χ1 ϕ1 ψ1 x0, σ1 = (χ1, ϕ1::ψ1) /\
+                                      contn ϕ1 = (c_stmt (s_rtrn x0))) \/
+                      (exists χ1 ϕ1 ψ1 x0 s, σ1 = (χ1, ϕ1::ψ1) /\
+                                        contn ϕ1 = (c_stmt (s_stmts (s_rtrn x0) s))).
+Proof.
+  intros M σ1 σ2 Hred;
+    induction Hred;
+    intros;
+    try solve [left; repeat eexists; eauto with loo_db];
+    try solve [right; left; repeat eexists; eauto with loo_db];
+    try solve [right; right; repeat eexists; eauto with loo_db].
+
+  - subst.
+    apply class_of_same_variable_map
+      with
+        (χ:=χ)(ϕ:=frm (update x v (vMap ϕ)) (c_stmt s))
+        (ψ:=ψ)(ϕ':=update_ϕ_map ϕ x v)(ψ':=ψ)
+      in H9;
+      auto.
+    assert (Htmp : (χ, update_ϕ_map ϕ x v :: ψ) = update_σ_map (χ, ϕ::ψ) x v);
+      [auto|rewrite Htmp in H9].
+    match goal with
+    | [H : classOf ?x (update_σ_map _ ?y _) _,
+       Hneq : ?y <> ?x |- _] =>
+      apply class_of_update in H;
+        auto
+    end.
+    match goal with
+    |[C1 : cls, C2 : cls, H : C1 <> C2 |- _] =>
+     contradiction H; subst
+    end.
+    eauto with loo_db.
+
+  -  match goal with
+     |[C1 : cls, C2 : cls, H : C1 <> C2 |- _] =>
+      contradiction H; subst
+     end.
+     eapply class_of_same_variable_map with (ϕ':=ϕ)(ψ':=ψ) in H12; eauto.
+     eapply class_of_update_same_cname in H12; eauto.
+
+  - match goal with
+    |[C1 : cls, C2 : cls, H : C1 <> C2 |- _] =>
+     contradiction H; subst
+    end.
+    apply (class_of_update_vMap this) with (ϕ':=ϕ)(y:=x)(v:=v_addr α) in H10;
+      auto.
+    apply class_of_update_heap_fresh with (C:=C1) in H10; eauto.
+  
+Qed.
+
+Lemma wf_config_this_has_class :
+  forall σ, σ_wf σ ->
+       exists C, classOf this σ C.
+Proof.
+  intros.
+  inversion H; subst.
+  inversion H0; subst.
+  destruct H2 as [ϕ Htmp];
+    destruct Htmp as [ψ'];
+    simpl in *;
+    andDestruct;
+    subst.
+  specialize (H4 ϕ (in_eq ϕ ψ')).
+  inversion H4; subst.
+  destruct H2 as [α Htmp];
+    destruct Htmp as [o];
+    andDestruct.
+  exists (cname o).
+  eapply cls_of; eauto.
+  eapply int_x; simpl; eauto.
+Qed.
+
+Lemma reductions_implies_method_call_or_rtrn :
+  forall M1 M2 σ1 σ2, M1 ⦂ M2 ⦿ σ1 ⤳… σ2 ->
+                 σ_wf σ1 ->
+                 (exists χ1 ϕ1 ψ1 x0 y0 m ps s, σ1 = (χ1, ϕ1::ψ1) /\
+                                           contn ϕ1 = (c_stmt (s_stmts (s_meth x0 y0 m ps) s))) \/
+                 (exists χ1 ϕ1 ψ1 x0, σ1 = (χ1, ϕ1::ψ1) /\
+                                 contn ϕ1 = (c_stmt (s_rtrn x0))) \/
+                 (exists χ1 ϕ1 ψ1 x0 s, σ1 = (χ1, ϕ1::ψ1) /\
+                                   contn ϕ1 = (c_stmt (s_stmts (s_rtrn x0) s))).
+Proof.
+  intros.
+  induction H; subst; auto.
+
+  destruct (wf_config_this_has_class σ H0) as [C].
+  assert (Hwf : σ_wf σ');
+    [eapply reduction_preserves_config_wf; eauto|].
+  destruct (wf_config_this_has_class σ' Hwf) as [C'].
+  repeat match goal with
+         | [Ha : forall _ : cls, classOf this ?σ _ -> _,
+              Hb : classOf this ?σ ?C |- _] =>
+           specialize (Ha C Hb)
+         end.
+  eapply reduction_different_classes_implies_method_call_or_rtrn; eauto.
+  intro Hcontra;
+    subst;
+    crush.
+Qed.
+
+Lemma pair_reduction_change_implies_method_call :
+  forall M1 M2 σ1 σ2, M1 ⦂ M2 ⦿ σ1 ⤳ σ2 ->
+                 σ_wf σ1 ->
+                 (exists χ1 ϕ1 ψ1 x0 y0 m ps s, σ1 = (χ1, ϕ1::ψ1) /\
+                                           contn ϕ1 = (c_stmt (s_stmts (s_meth x0 y0 m ps) s))) \/
+                 (exists χ1 ϕ1 ψ1 x0, σ1 = (χ1, ϕ1::ψ1) /\
+                                 contn ϕ1 = (c_stmt (s_rtrn x0))) \/
+                 (exists χ1 ϕ1 ψ1 x0 s, σ1 = (χ1, ϕ1::ψ1) /\
+                                   contn ϕ1 = (c_stmt (s_stmts (s_rtrn x0) s))).
+Proof.
+  intros.
+  induction H;
+    subst.
+  eapply reductions_implies_method_call_or_rtrn; eauto.
+Qed.
+
+Lemma was_change :
+  (forall M1 M2 σ A, M1 ⦂ M2 ◎ σ ⊨ A ->
+                M1 ⦂ M2 ◎ σ ⊨ (a_was (¬ A)) ->
+                M1 ⦂ M2 ◎ σ ⊨ (a_was (¬ A ∧ (a_next A)))) /\
+  (forall M1 M2 σ A, M1 ⦂ M2 ◎ σ ⊭ A ->
+                M1 ⦂ M2 ◎ σ ⊭ (a_was (¬ A)) ->
+                M1 ⦂ M2 ◎ σ ⊭ (a_was (¬ A ∧ (a_next A)))).
+Proof.
+Admitted.
+
+Lemma was_conjunction :
+  forall A1 A2, entails (a_was (A1 ∧ A2))
+                   ((a_was A1) ∧ (a_was A2)).
+Proof.
+  intros.
+  apply ent;
+    intros;
+    repeat (a_prop).
+
+  - match goal with
+    | [H : _ ⦂ _ ◎ _ ⊨ (a_was (_ ∧ _)) |- _] =>
+      inversion H; subst
+    end.
+    apply sat_was;
+      intros.
+    match goal with
+    | [ Ha : initial ?σ0,
+             Hb : ?M1 ⦂ ?M2 ⦿ ?σ0 ⤳⋆ ?σ',
+                  Hc : forall σ, initial σ ->
+                            ?M1 ⦂ ?M2 ⦿ σ ⤳⋆ ?σ' ->  _ |- exists _ : config, _ ] =>
+      specialize (Hc σ0 Ha Hb);
+        let someσ1 := fresh "σ" in
+        let someσ2 := fresh "σ" in
+        let Htmp := fresh in
+        destruct Hc as [someσ1 Htmp];
+          destruct Htmp as [someσ2];
+          exists someσ1, someσ2;
+          intros
+    end.
+    andDestruct; a_prop.
+    repeat split; eauto with loo_db.
+
+  - match goal with
+    | [H : _ ⦂ _ ◎ _ ⊨ (a_was (_ ∧ _)) |- _] =>
+      inversion H; subst
+    end.
+    apply sat_was;
+      intros.
+    match goal with
+    | [ Ha : initial ?σ0,
+             Hb : ?M1 ⦂ ?M2 ⦿ ?σ0 ⤳⋆ ?σ',
+                  Hc : forall σ, initial σ ->
+                            ?M1 ⦂ ?M2 ⦿ σ ⤳⋆ ?σ' ->  _ |- exists _ : config, _ ] =>
+      specialize (Hc σ0 Ha Hb);
+        let someσ1 := fresh "σ" in
+        let someσ2 := fresh "σ" in
+        let Htmp := fresh in
+        destruct Hc as [someσ1 Htmp];
+          destruct Htmp as [someσ2];
+          exists someσ1, someσ2;
+          intros
+    end.
+    andDestruct; a_prop.
+    repeat split; eauto with loo_db.
+Qed.
+
+Hint Resolve was_conjunction : chainmail_db.
+Hint Rewrite was_conjunction : chainmail_db.
+
+Lemma pair_reductions_trans :
+  forall M1 M2 σ1 σ2, M1 ⦂ M2 ⦿ σ1 ⤳⋆ σ2 ->
+                 forall σ3, M1 ⦂ M2 ⦿ σ2 ⤳⋆ σ3 ->
+                       M1 ⦂ M2 ⦿ σ1 ⤳⋆ σ3.
+Proof.
+  intros M1 M2 σ1 σ2 Hred;
+    induction Hred;
+    intros;
+    eauto with loo_db.
+Qed.
+
+Hint Resolve pair_reductions_trans : loo_db.
+Hint Rewrite pair_reductions_trans : loo_db.
+
+Lemma finite_ψ_top_frame :
+  forall ϕ ψ, finite_ψ (ϕ::ψ) ->
+         finite_ψ (ϕ::nil).
+Proof.
+  intros.
+  finite_auto;
+    intros.
+  inversion H0; subst.
+
+  - apply H, in_eq.
+
+  - crush.
+
+Qed.
+
+Hint Resolve finite_ψ_top_frame : loo_db.
+
+Lemma finite_σ_top_frame :
+  forall χ ϕ ψ, finite_σ (χ, ϕ::ψ) ->
+           forall χ', finite_σ (χ', ϕ::nil).
+Proof.
+  intros.
+  unfold finite_σ in *;
+    simpl in *.
+  eauto with loo_db.
+Qed.
+
+Hint Resolve finite_σ_top_frame : loo_db.
+
+Lemma has_self_σ_top_frame :
+  forall χ ϕ ψ, has_self_σ (χ, ϕ::ψ) ->
+           has_self_σ (χ, ϕ::nil).
+Proof.
+  intros.
+  inversion H; subst.
+  apply self_config; intros.
+  inversion H0; subst.
+
+  - apply H1, in_eq.
+
+  - crush.
+Qed.
+
+Hint Resolve has_self_σ_top_frame : loo_db.
+
+Lemma not_stuck_σ_top_frame :
+  forall χ ϕ ψ, not_stuck_σ (χ, ϕ::ψ) ->
+           not_stuck_σ (χ, ϕ::nil).
+Proof.
+  intros.
+  inversion H; subst.
+  unfold not_stuck_σ.
+  destruct_exists_loo;
+    simpl in *;
+    andDestruct.
+  crush.
+  repeat eexists; eauto.
+Qed.
+
+Hint Resolve not_stuck_σ_top_frame : loo_db.
+
+Lemma waiting_σ_top_frame :
+  forall χ ϕ ψ, waiting_σ (χ, ϕ::ψ) ->
+           waiting_σ (χ, ϕ::nil).
+Proof.
+  intros.
+  inversion H; subst.
+  unfold waiting_σ.
+  destruct_exists_loo;
+    simpl in *;
+    andDestruct.
+  crush.
+  repeat eexists; eauto.
+  unfold waiting_ψ;
+    intros;
+    crush.
+Qed.
+
+Hint Resolve waiting_σ_top_frame : loo_db.
+
+Lemma σ_wf_top_frame :
+  forall χ ϕ ψ, σ_wf (χ, ϕ::ψ) ->
+           σ_wf (χ, ϕ::nil).
+Proof.
+  intros.
+  inversion H; subst.
+  apply config_wf; eauto with loo_db.
+Qed.
+
+Hint Resolve σ_wf_top_frame : loo_db.
+
+Lemma finite_ϕ_update :
+  forall ϕ, finite_ϕ ϕ ->
+       forall y v, finite_ϕ (update_ϕ_map ϕ y v).
+Proof.
+  intros.
+  finite_auto;
+    intros.
+  destruct ϕ as [m c];
+    simpl in *.
+  eauto with map_db.
+Qed.
+
+Hint Resolve finite_ϕ_update : loo_db.
+
+Lemma finite_ψ_update :
+  forall ψ, finite_ψ ψ ->
+       forall y v, finite_ψ (update_ψ_map ψ y v).
+Proof.
+  intros.
+  unfold finite_ψ in *;
+    intros.
+  destruct ψ as [|ϕ' ψ'];
+    simpl in *;
+    [crush|].
+  destruct H0; subst;
+    eauto with loo_db.
+Qed.
+
+Hint Resolve finite_ψ_update : loo_db.
+
+Lemma finite_σ_update :
+  forall σ, finite_σ σ ->
+       forall y v, finite_σ (update_σ_map σ y v).
+Proof.
+  intros.
+  unfold finite_σ in *;
+    simpl in *;
+    eauto with loo_db.
+Qed.
+
+Hint Resolve finite_σ_update : loo_db.
+
+Lemma has_self_σ_update :
+  forall σ, has_self_σ σ ->
+       forall y v A, fresh_x_σ y σ A ->
+                has_self_σ (update_σ_map σ y v).
+Proof.
+  intros.
+  inversion H; subst.
+  apply self_config;
+    intros;
+    simpl in *.
+  destruct ψ as [|ϕ' ψ'];
+    unfold update_ψ_map in *;
+    unfold update_ϕ_map in *;
+    [crush|].
+  destruct H2;
+    subst;
+    eauto.
+
+  - apply self_frm.
+    specialize (H1 ϕ' (in_eq ϕ' ψ')).
+    inversion H1;
+      subst.
+    repeat destruct_exists_loo;
+      andDestruct;
+      crush.
+    exists α, o;
+      split;
+      auto.
+    destruct (eq_dec y this) as [Heq|Hneq];
+      subst;
+      repeat map_rewrite;
+      eq_auto.
+    unfold fresh_x_σ in *;
+      repeat destruct_exists_loo;
+      andDestruct;
+      match goal with
+      | [H : (_, _) = (_, _) |- _] =>
+        inversion H; subst
+      end.
+    match goal with
+    | [H : fresh_x _ _ _ |- _] =>
+      inversion H;
+        crush
+    end.
+
+  - apply H1, in_cons; auto.
+Qed.
+
+Hint Resolve has_self_σ_update : loo_db.
+
+Lemma not_stuck_σ_update :
+  forall σ, not_stuck_σ σ ->
+       forall y v, not_stuck_σ (update_σ_map σ y v).
+Proof.
+  intros.
+  inversion H; subst.
+  unfold not_stuck_σ.
+  destruct_exists_loo;
+    simpl in *;
+    andDestruct.
+  crush.
+  repeat eexists; eauto.
+Qed.
+
+Hint Resolve not_stuck_σ_update : loo_db.
+
+Lemma waiting_σ_update :
+  forall σ, waiting_σ σ ->
+       forall y v, waiting_σ (update_σ_map σ y v).
+Proof.
+  intros.
+  inversion H; subst.
+  unfold waiting_σ.
+  destruct_exists_loo;
+    simpl in *;
+    andDestruct.
+  crush.
+  repeat eexists; eauto.
+Qed.
+
+Hint Resolve waiting_σ_update : loo_db.
+
+Lemma σ_wf_update :
+  forall σ, σ_wf σ ->
+       forall y v A, fresh_x_σ y σ A ->
+                σ_wf (update_σ_map σ y v).
+Proof.
+  intros.
+  inversion H; subst.
+  apply config_wf; eauto with loo_db.
+Qed.
+
+Hint Resolve σ_wf_update : loo_db.
+
+Lemma has_self_σ_this_interpretation :
+  forall χ ϕ ψ, has_self_σ (χ, ϕ::ψ) ->
+           exists α o, ⌊ this ⌋ (χ, ϕ::ψ) ≜ (v_addr α) /\
+                  χ α = Some o.
+Proof.
+  intros.
+  match goal with
+  | [H : has_self_σ ?σ |- _] =>
+    inversion H; subst
+  end.
+  match goal with
+  | [H : forall ϕ, In ϕ (?ϕ::?ψ) -> _ |- _] =>
+    specialize (H ϕ (in_eq ϕ ψ));
+      inversion H;
+      subst
+  end.
+  repeat destruct_exists_loo;
+    andDestruct.
+  exists α, o; split; eauto.
+  eapply int_x; simpl; eauto.
+Qed.
+
+Hint Resolve has_self_σ_this_interpretation : loo_db.
+
+Lemma wf_σ_this_interpretation :
+  forall χ ϕ ψ, σ_wf (χ, ϕ::ψ) ->
+           exists α o, ⌊ this ⌋ (χ, ϕ::ψ) ≜ (v_addr α) /\
+                  χ α = Some o.
+Proof.
+  intros χ ϕ ψ H;
+    inversion H;
+    subst;
+    eauto with loo_db.
+Qed.
+
+Hint Resolve wf_σ_this_interpretation : loo_db.
+
+Lemma update_map_implies_mapping :
+  forall {A B : Type}`{Eq A} (f : partial_map A B) a b,
+    f a = Some b ->
+    forall a' b', exists b'', (update a' b' f) a = Some b''.
+Proof.
+  intros.
+  repeat map_rewrite.
+  destruct (eq_dec a a');
+    subst;
+    eq_auto;
+    eexists;
+    eauto.
+Qed.
+
+Hint Resolve update_map_implies_mapping : map_db.
+
+Lemma reduction_heap_monotonic :
+  forall M σ1 σ2, M ∙ σ1 ⤳ σ2 ->
+             forall α o, (fst σ1) α = Some o ->
+                    exists o', (fst σ2) α = Some o'.
+Proof.
+  intros M σ1 σ2 Hred;
+    induction Hred;
+    intros;
+    subst;
+    simpl in *;
+    eauto with map_db.
+Qed.
+
+Hint Resolve reduction_heap_monotonic : loo_db.
+
+Lemma reductions_heap_monotonic :
+  forall M1 M2 σ1 σ2, M1 ⦂ M2 ⦿ σ1 ⤳… σ2 ->
+                 forall α o, (fst σ1) α = Some o ->
+                        exists o', (fst σ2) α = Some o'.
+Proof.
+  intros M1 M2 σ1 σ2 Hred;
+    induction Hred;
+    intros;
+    eauto with loo_db.
+  match goal with
+  | [Ha : forall α' o', fst ?σ1 α' = Some o' -> exists o'', _,
+       Hb : fst ?σ1 ?α = Some ?o |- _] =>
+    specialize (Ha α o Hb)
+  end.
+  destruct_exists_loo.
+  eauto with loo_db.
+Qed.
+
+Hint Resolve reductions_heap_monotonic : loo_db.
+
+Lemma pair_reduction_heap_monotonic :
+  forall M1 M2 σ1 σ2, M1 ⦂ M2 ⦿ σ1 ⤳ σ2 ->
+                 forall α o, (fst σ1) α = Some o ->
+                        exists o', (fst σ2) α = Some o'.
+Proof.
+  intros M1 M2 σ1 σ2 Hred;
+    induction Hred;
+    intros;
+    eauto with loo_db.
+Qed.
+
+Hint Resolve pair_reduction_heap_monotonic.
+
+Lemma pair_reductions_heap_monotonic :
+  forall M1 M2 σ1 σ2, M1 ⦂ M2 ⦿ σ1 ⤳⋆ σ2 ->
+                 forall α o, (fst σ1) α = Some o ->
+                        exists o', (fst σ2) α = Some o'.
+Proof.
+  intros M1 M2 σ1 σ2 Hred;
+    induction Hred;
+    intros;
+    eauto with loo_db.
+  destruct (pair_reduction_heap_monotonic M1 M2 σ1 σ H α o) as [o'];
+    auto.
+  match goal with
+  | [Ha : forall α' o', fst ?σ α' = Some o' -> exists o'', _,
+       Hb : fst ?σ ?α = Some ?o |- _] =>
+    specialize (Ha α o Hb)
+  end.
+  destruct_exists_loo.
+  eauto with loo_db.
+Qed.
+
+Hint Resolve pair_reductions_heap_monotonic : loo_db.
+
+Lemma has_self_adaptation :
+  forall σ1 σ2, has_self_σ σ1 ->
+           has_self_σ σ2 ->
+           forall σ, σ1 ◁ σ2 ≜ σ ->
+                (forall α o, (fst σ1) α = Some o ->
+                        exists o', (fst σ2) α = Some o') ->
+                has_self_σ σ.
+Proof.
+  intros; subst.
+  match goal with
+  | [H : ?σ1 ◁ ?σ2 ≜ ?σ |- _] =>
+    inversion H;
+      subst
+  end.
+  repeat match goal with
+         | [H : has_self_σ (?χ, ?ψ)  |- _] =>
+           notHyp (forall ϕ : frame, In ϕ ψ -> has_self_ϕ χ ϕ);
+             inversion H; subst
+         end.
+  apply self_config;
+    intros ϕ Hin;
+    destruct Hin;
+    subst.
+
+  - repeat match goal with
+           | [H : forall ϕ' : frame, In ϕ' (?ϕ::?ψ) -> has_self_ϕ _ _ |- _] =>
+             specialize (H ϕ (in_eq ϕ ψ));
+               inversion H;
+               subst
+           end.
+    repeat destruct_exists_loo;
+      andDestruct;
+      repeat match goal with
+             | [H : context [vMap _] |- _] =>
+               simpl in H
+             end.
+    apply self_frm;
+      simpl.
+    unfold fst in *.
+    match goal with
+    |[Ha : forall α' o', ?χ α' = Some o' -> exists _, _,
+        Hb : ?χ ?α = Some ?o |- _] =>
+     specialize (Ha α o Hb)
+    end.
+    repeat destruct_exists_loo.
+    exists α0, o1;
+      split; auto.
+    apply extend_some_2; auto.
+    apply disjoint_dom_symmetry.
+    apply disjoint_composition; eauto with map_db.
+
+  - match goal with
+    | [Ha : forall ϕ', In ϕ' (_::?ψ) -> has_self_ϕ ?χ' ϕ',
+         Hb : In ?ϕ ?ψ |- has_self_ϕ ?χ' ?ϕ] =>
+      apply Ha, in_cons; auto
+    end.
+Qed.
+
+Hint Resolve has_self_adaptation : loo_db.
+
+Lemma extend_update :
+  forall {A B : Type}`{Eq A}(f g : partial_map A B) a b,
+    (update a b f) ∪ g = (update a b (f ∪ g)).
+Proof.
+  intros;
+    unfold extend;
+    repeat map_rewrite;
+    apply functional_extensionality;
+    intros a';
+    destruct (eq_dec a' a);
+    subst;
+    eq_auto.
+Qed.
+
+Hint Resolve extend_update : map_db.
+Hint Rewrite @extend_update : map_db.
+
+Lemma finite_extend :
+  forall {A B : Type}`{Eq A}(f : partial_map A B),
+    finite f ->
+    forall g, finite g ->
+         finite (f ∪ g).
+Proof.
+  intros A B HeqA f Hfin;
+    induction Hfin;
+    intros;
+    auto.
+  rewrite extend_update; eauto with map_db.
+Qed.
+
+Hint Resolve finite_extend.
+
+Lemma compose_empty_right :
+  forall {A B C : Type}`{Eq A}{HeqB : Eq B}(f : partial_map A B),
+    (f ∘ (@empty B C HeqB)) = empty.
+Proof.
+  intros;
+    apply functional_extensionality;
+    intros a;
+    repeat map_rewrite;
+    simpl;
+    destruct (f a);
+    auto.
+Qed.
+
+Hint Resolve compose_empty_right : map_db.
+Hint Rewrite @compose_empty_right : map_db.
+
+Lemma compose_empty_left :
+  forall {A B C : Type}{HeqA : Eq A}`{Eq B}(f : partial_map B C),
+    ((@empty A B HeqA) ∘ f) = empty.
+Proof.
+  intros;
+    simpl;
+    auto.
+Qed.
+
+Hint Resolve compose_empty_left : map_db.
+Hint Rewrite @compose_empty_left : map_db.
+
+Lemma finite_map_composition_2' :
+  forall {A B C : Type}`{Eq A}`{Eq B}(g : partial_map B C),
+    finite_normal_form g -> forall (f : partial_map A B), one_to_one f -> finite_normal_form (f ∘ g).
+Proof.
+  intros A B C HeqA HeqB g Hfin;
+    induction Hfin;
+    intros f H121.
+
+  - rewrite compose_empty_right; auto with map_db.
+
+  - destruct (excluded_middle (exists a', f a' = Some a)).
+    + destruct_exists_loo.
+      assert (Heq : f ∘ (update a b m) = (update x b (f ∘ m)));
+        [apply functional_extensionality; intros a'; simpl
+        |rewrite Heq; apply norm_update; auto; crush].
+      repeat map_rewrite; simpl.
+      destruct (partial_map_dec a' f) as [Hsome|Hnone];
+        [destruct Hsome as [b' Htmp];
+         rewrite Htmp
+        |rewrite Hnone].
+      * destruct (eq_dec b' a);
+          subst;
+          eq_auto.
+        ** destruct (eq_dec a' x);
+             subst;
+             eq_auto.
+           specialize (H121 x a' a H0 Htmp);
+             crush.
+        ** destruct (eq_dec a' x);
+             subst;
+             eq_auto.
+           crush.
+      * destruct (eq_dec a' x);
+          subst;
+          [crush|eq_auto].
+    + assert (Heq : f ∘ update a b m = f ∘ m);
+        [apply functional_extensionality; intros a';
+         simpl
+        |rewrite Heq; auto].
+      destruct (partial_map_dec a' f) as [Hsome|Hnone];
+        [destruct Hsome as [b' Hsome];
+         rewrite Hsome
+        |rewrite Hnone; auto].
+      repeat map_rewrite;
+        destruct (eq_dec a b');
+        subst;
+        eq_auto.
+      contradiction n; eauto.
+Qed.
+
+Hint Resolve finite_map_composition_2' : map_db.
+
+Lemma finite_map_composition_2 :
+  forall {A B C : Type}`{Eq A}`{Eq B}(g : partial_map B C),
+    finite g -> forall (f : partial_map A B), one_to_one f -> finite (f ∘ g).
+Proof.
+  intros; eauto with map_db.
+Qed.
+
+Hint Resolve finite_map_composition_2 : map_db.
+
+Lemma finite_adaptation :
+  forall σ1 σ2, finite_σ σ1 ->
+           finite_σ σ2 ->
+           forall σ, σ1 ◁ σ2 ≜ σ ->
+                finite_σ σ.
+Proof.
+  intros σ1 σ2 Hfin1 Hfin2 σ Hadapt;
+    inversion Hadapt;
+    subst.
+  unfold finite_σ, finite_ψ, finite_ϕ in *;
+    intros ϕ;
+    unfold snd in *;
+    intros Hin;
+    destruct Hin;
+    subst;
+    [unfold vMap|].
+
+  - repeat match goal with
+           | [H : forall ϕ', In ϕ' (?ϕ::?ψ) -> finite (vMap ϕ')  |- _] =>
+             specialize (H ϕ (in_eq ϕ ψ));
+               unfold vMap in H
+           end.
+    apply finite_extend;
+      auto.
+    apply finite_map_composition_2; auto.
+
+  - apply Hfin2, in_cons; auto.
+
+Qed.
+
+Hint Resolve finite_adaptation : loo_db.
+
+Lemma not_stuck_adaptation :
+  forall σ1 σ2, not_stuck_σ σ2 ->
+           forall σ, σ1 ◁ σ2 ≜ σ ->
+                not_stuck_σ σ.
+Proof.
+  intros.
+  match goal with
+  | [H : ?σ1 ◁ ?σ2 ≜ ?σ |- _] =>
+    inversion H; subst
+  end.
+  unfold not_stuck_σ, snd in *.
+  repeat destruct_exists_loo;
+    andDestruct.
+  match goal with
+  | [H : ?ϕ1::?ψ  = ?ϕ2::?ψ2 |- _] =>
+    inversion H; subst
+  end.
+  exists (frm ((f ∘ β') ∪ β) (c_stmt (❲ f' ↦ s ❳))), ψ0;
+    split; auto.
+  unfold not_stuck_ϕ, contn in *.
+  auto with loo_db.
+Qed.
+
+Hint Resolve not_stuck_adaptation : loo_db.
+
+Lemma waiting_adaptation :
+  forall σ1 σ2, waiting_σ σ2 ->
+           forall σ, σ1 ◁ σ2 ≜ σ ->
+                waiting_σ σ.
+Proof.
+  intros.
+  match goal with
+  | [H : ?σ1 ◁ ?σ2 ≜ ?σ |- _] =>
+    inversion H; subst
+  end.
+  unfold waiting_σ, snd in *.
+  repeat destruct_exists_loo;
+    andDestruct.
+  match goal with
+  | [H : ?ϕ1::?ψ  = ?ϕ2::?ψ2 |- _] =>
+    inversion H; subst
+  end.
+  eexists; eauto.
+Qed.
+
+Hint Resolve waiting_adaptation : loo_db.
+
+Lemma wf_adaptation :
+  forall σ1 σ2, σ_wf σ1 ->
+           σ_wf σ2 ->
+           forall σ, σ1 ◁ σ2 ≜ σ ->
+                (forall α o, (fst σ1) α = Some o ->
+                        exists o', (fst σ2) α = Some o') ->
+                σ_wf σ.
+Proof.
+  intros;
+    match goal with
+    | [Ha : σ_wf ?σ1,
+            Hb : σ_wf ?σ2 |- _] =>
+      inversion Ha;
+        inversion Hb;
+        subst
+    end.
+  apply config_wf; eauto with loo_db.
+Qed.
+
+Hint Resolve wf_adaptation : loo_db.
+
+Lemma guards_method_call :
+  forall M1 M2 σ1 σ2, M1 ⦂ M2 ⦿ σ1 ⤳ σ2 ->
+                 forall χ ϕ σ1' σ2', (χ, ϕ::nil) ◁ σ1 ≜ σ1' ->
+                                (χ, ϕ::nil) ◁ σ2 ≜ σ2' ->
+                                σ_wf (χ, ϕ::nil) ->
+                                M1 ⦂ M2 ⦿ (χ, ϕ::nil) ⤳⋆ σ1 ->
+                                forall x y, M1 ⦂ M2 ◎ σ1' ⊨ guards x y ->
+                                       M1 ⦂ M2 ◎ σ2' ⊨ (¬ guards x y) ->
+                                       (forall σ σ', M1 ⦂ M2 ⦿ (χ, ϕ::nil) ⤳⋆ σ ->
+                                                M1 ⦂ M2 ⦿ σ ⤳⋆ σ1 ->
+                                                (χ, ϕ::nil) ◁ σ ≜ σ' ->
+                                                M1 ⦂ M2 ◎ σ' ⊨ guards x y) ->
+                                       (M1 ⦂ M2 ◎ (χ, ϕ::nil) ⊨ guards x y) ->
+                                       exists z m vMap, M1 ⦂ M2 ◎ σ1' ⊨ ((a_ this) calls (a_ z) ∎ m ⟨ vMap ⟩).
+Proof.
+  intros.
+
+  destruct (pair_reduction_change_implies_method_call M1 M2 σ1 σ2);
+    auto.
+
+  - eapply pair_reductions_preserves_config_wf;
+      eauto.
+
+  - repeat destruct_exists_loo;
+      andDestruct;
+      subst.
+    match goal with
+    | [H : (_, _) ◁ (_, _) ≜ _ |- _] =>
+      inversion H; subst
+    end;
+      repeat (match goal with
+              | [Heq : ?x = ?x |- _] =>
+                clear Heq
+              | [H : (_, _) = (_, _) |- _] =>
+                inversion H; subst
+              end).
+    match goal with
+    | [H : context [contn _] |- _] =>
+      simpl in H
+    end.
+    match goal with
+    | [H : c_stmt _ = c_stmt _ |- _] =>
+      inversion H; subst
+    end.
+    rename_simpl.
+    let α := fresh "α" in
+    let o := fresh "o" in
+    let H := fresh in
+    destruct (wf_σ_this_interpretation χ')
+      with
+        (ψ:=ψ')
+        (ϕ:=frm ((f ∘ β') ∪ β)
+                (c_stmt (s_stmts (s_meth (❲ f' ↦ x0 ❳) (❲ f' ↦ x1 ❳) m (❲ f' ↦ vMap ❳)) (❲ f' ↦ s ❳))))
+      as [α H];
+      auto.
+    +  apply (wf_adaptation)
+         with
+           (σ1:= (χ1, (frm β c) :: nil))
+           (σ2:= (χ', (frm β' (c_stmt (s_stmts (s_meth x0 x1 m vMap) s))) :: ψ'));
+         auto.
+       * eapply pair_reductions_preserves_config_wf;
+           eauto.
+       * intros.
+         eapply pair_reductions_heap_monotonic; eauto.
+
+    + destruct_exists_loo; andDestruct.
+      exists (❲ f' ↦ x1 ❳), m, (❲ f' ↦ vMap ❳ ∘ v_to_av).
+      eapply sat_call
+        with (χ:=χ')(ψ:=ψ')
+             (x':=❲ f' ↦ x0 ❳)
+             (y':=❲ f' ↦ x1 ❳)
+             (vMap':=❲ f' ↦ vMap ❳)
+             (s:=❲ f' ↦ s ❳);
+        eauto.
+      * admit. (* x1 maps to something  *)
+      * admit. (* x1 maps to something  *)
+      * admit. (* same domain refl *)
+      * intros.
+        (* vMap, the parameters supplied to the method call maps to some values in the  *)
+        (* this perhaps needs to be added to the reduction definition *)
+        admit.
+
+  - admit.
+    (* if the continuation is a return statement, 
+       then there is some method call from within M1 that is  
+       being returned from.
+       Subsequently, either some method then returns back to 
+       client code, or client code is called from the module in 
+       question.
+
+     *)
+
+Admitted.
+
+(** 
+
+#<h2>#Thoughts on access, expose, temporal operators:#</h2>#
+
+ *)
+
+(**
+
+The non-determinism of both was and will means that
+will(was _) and was(will _) have no relation to 
+the current configuration. In the original version 
+of the expose example, we used *)
+(**will((_ access _) ⇒ was (_)). *)
+(**
+This does not mean what we expect it to mean, because
+the "was" does not only refer to the reduction from the 
+current configuration to the future moment in time 
+where the data was exposed, rather it refers to all 
+possible reductions that lead up to the future point in 
+time. What we really intend to say is "if in some future
+point in time, the private data is aliased, then 
+at some point in time between the current moment and that 
+future moment, the expose method must have been called".
+
+ *)
+(**
+
+In the current model, only was is non-deterministic, 
+will is deterministic. As such was(will _) does in fact
+mean what we initially meant it to mean, however, 
+ideally we would like to model non-determinism of reduction 
+to cover really world programs.
+
+ *)
