Coq/linking_properties.v
@@ -1,0 +1,268 @@
+Require Import common.
+Require Import loo_def.
+Require Import loo_properties.
+Require Import List.
+Require Import String.
+Open Scope string_scope.
+Require Import CpdtTactics.
+Require Import Coq.Logic.FunctionalExtensionality.
+
+(** Properties of Linking *)
+Lemma moduleLinking_associative :
+  forall M1 M2 M12, M1 ⋄ M2 ≜ M12 ->
+               forall M3 M23, M2 ⋄ M3 ≜ M23 ->
+                         forall M M', M12 ⋄ M3 ≜ M ->
+                                 M1 ⋄ M23 ≜ M' ->
+                                 M = M'.
+Proof.
+  intros.
+  inversion H;
+    inversion H0;
+    inversion H1;
+    inversion H2;
+    subst.
+
+  apply functional_extensionality;
+    intro C.
+  remember (M1 C) as res1;
+    remember (M2 C) as res2;
+    remember (M3 C) as res3.
+  destruct res1 as [CDef1|];
+    destruct res2 as [CDef2|];
+    destruct res3 as [CDef3|];
+    unfold extend;
+    rewrite <- Heqres1;
+    auto.
+Qed.
+
+Lemma moduleLinking_commutative_1 :
+  forall M1 M2 M, M1 ⋄ M2 ≜ M ->
+             M_wf M1 ->
+             M_wf M2 ->
+             M2 ⋄ M1 ≜ M.
+Proof.
+  intros.
+  inversion H;
+    subst.
+
+  assert (Hrewrite : extend M1 M2 = extend M2 M1);
+    [|rewrite Hrewrite; apply m_link; eauto].
+  
+  apply functional_extensionality;
+    intro C.
+  unfold extend.
+  remember (M1 C) as r1;
+    remember (M2 C) as r2;
+    destruct r1 as [def1|];
+    destruct r2 as [def2|];
+    eauto.
+  destruct (eq_dec C ObjectName) as [|Hneq];
+    [subst|].
+  inversion H0;
+    inversion H1;
+    subst;
+    crush.
+
+  rewrite H2 with (def:=def1) in Heqr2;
+    crush.
+Qed.
+
+Lemma moduleLinking_commutative_2 :
+  forall M1 M2 M, M1 ⋄ M2 ≜ M ->
+             forall M', M2 ⋄ M1 ≜ M' ->
+                   M_wf M1 ->
+                   M_wf M2 ->
+                   M = M'.
+Proof.
+  intros.
+  inversion H;
+    inversion H0;
+    subst.
+
+  apply functional_extensionality;
+    intros C.
+  unfold extend.
+  remember (M1 C) as res1;
+    remember (M2 C) as res2.
+  destruct res1 as [CDef1|];
+    destruct res2 as [CDef2|];
+    auto.
+  destruct (eq_dec C ObjectName) as [|Hneq];
+    [subst|].
+  inversion H1;
+    inversion H2;
+    subst.
+  rewrite <- Heqres1 in H5;
+    rewrite <- Heqres2 in H11.
+  inversion H5;
+    inversion H11;
+    auto.
+  symmetry in Heqres1;
+    apply H9 in Heqres1.
+  rewrite Heqres1 in Heqres2;
+    crush.
+  apply H3 in Heqres1;
+    auto.
+Qed.
+
+Lemma linking_preserves_reduction :
+  forall M1 σ1 σ2, M1 ∙ σ1 ⤳ σ2 ->
+              forall M2 M, M1 ⋄ M2 ≜ M ->
+                      M ∙ σ1 ⤳ σ2.
+Proof.
+  intros M1 σ1 σ2 Hred;
+    induction Hred;
+    intros;
+    subst;
+    eauto with loo_db.
+
+  - eapply r_mth;
+      eauto.
+    inversion H9;
+      subst;
+      unfold extend in *;
+      eauto.
+    rewrite H4;
+      auto.
+
+  - eapply r_new;
+      eauto.
+    inversion H9;
+      unfold extend in *;
+      subst;
+      eauto.
+    rewrite H3;
+      auto.
+Qed.
+
+(*Lemma linking_preserves_reductions :
+  forall M1 M2 σ1 σ2, M1 ⦂ M2 ⦿ σ1 ⤳… σ2 ->
+                 forall M3 M', M1 ∘ M3 ≜ M' ->
+                          forall M4 M'', M2 ∘ M4 ≜ M'' ->
+                                    M_wf M1 ->
+                                    M_wf M2 ->
+                                    M_wf M3 ->
+                                    M_wf M4 ->
+                                    (exists M''', M' ∘ M'' ≜ M''') ->
+                                    M' ⦂ M'' ⦿ σ1 ⤳… σ2.
+Proof.
+  intros M1 M2 σ1 σ2 Hred;
+    induction Hred;
+    intros;
+    eauto.
+  inversion H3;
+    inversion H4;
+    subst.
+  destruct H9 as [M'''].
+  apply pr_single with (M:=M''');
+    intros;
+    eauto.
+  inversion H9;
+    subst.
+  apply linking_preserves_reduction
+    with (M1:=extend M1 M2)
+         (M2:=extend M3 M4);
+    auto.
+  inversion H;
+    subst;
+    auto.
+  assert (Hrewrite : extend (extend M1 M2) (extend M3 M4) = extend (extend M1 M3) (extend M2 M4));
+    [|rewrite <- Hrewrite; auto; apply m_link; intros].
+  apply functional_extensionality;
+    intros C.
+  remember (M1 C) as res1;
+    remember (M2 C) as res2;
+    remember (M3 C) as res3;
+    remember (M4 C) as res4.
+  destruct (eq_dec C ObjectName) as [|Hneq];
+    [subst C
+    |].
+  unfold extend;
+    destruct res1 as [Cdef1|];
+    destruct res2 as [Cdef2|];
+    destruct res3 as [Cdef3|];
+    destruct res4 as [Cdef4|];
+    rewrite <- Heqres1;
+    try rewrite <- Heqres2;
+    try rewrite <- Heqres3;
+    try rewrite <- Heqres4;
+    auto.
+
+  inversion H5; subst; crush.
+  rewrite Heqres2, Heqres3;
+    inversion H6;
+    inversion H7;
+    subst.
+  rewrite H14, H19;
+    auto.
+
+  unfold extend;
+    destruct res1 as [Cdef1|];
+    destruct res2 as [Cdef2|];
+    destruct res3 as [Cdef3|];
+    destruct res4 as [Cdef4|];
+    rewrite <- Heqres1;
+    try rewrite <- Heqres2;
+    try rewrite <- Heqres3;
+    try rewrite <- Heqres4;
+    auto.
+  assert (Hclass : extend M1 M3 C = Some Cdef3);
+    [unfold extend; rewrite <- Heqres1; auto|].
+  apply H12 in Hclass;
+    auto;
+    unfold extend in Hclass;
+    rewrite <- Heqres2 in Hclass;
+    crush.
+  assert (Hclass : extend M1 M3 C = Some Cdef3);
+    [unfold extend; rewrite <- Heqres1; auto|].
+  apply H12 in Hclass;
+    auto;
+    unfold extend in Hclass;
+    rewrite <- Heqres2 in Hclass;
+    crush.
+
+  unfold extend in H17;
+    remember (M1 C) as res1;
+    destruct res1 as [Cdef1|].
+  assert (M3 C = None);
+    [apply H10 with (def:=Cdef1); eauto|].
+  remember (M4 C) as res4;
+    destruct res4 as [Cdef4|];
+    symmetry in Heqres4.
+  assert (Htmp : extend M1 M3 C = Some Cdef1);
+    [unfold extend; rewrite <- Heqres1; auto|apply H12 in Htmp; auto].
+  unfold extend in Htmp.
+  rewrite Heqres4 in Htmp.
+  destruct (M2 C);
+    crush.
+  unfold extend;
+    crush.
+  assert (M4 C = None);
+    [apply H15 with (def:=def); auto| ].
+  assert (extend M1 M3 C = None);
+    [apply H13 with (def:= def); unfold extend; auto; rewrite H17; auto
+    |].
+  unfold extend in H19;
+    rewrite <- Heqres1 in H19.
+  unfold extend; rewrite H19, H18;
+    auto.
+  admit.
+  admit.
+
+  apply H2 in H12;
+    destruct H12 as [def];
+    exists def;
+    unfold extend;
+    crush.
+
+  destruct H8 as [M'''].
+  eapply pr_trans with (M:=M''');
+    eauto.
+  inversion H8;
+    subst;
+    auto.
+  inversion H;
+    subst.
+  
+  
+Abort.*)
