Coq/loo_reduction_properties.v
@@ -1,0 +1,1045 @@
+Require Import common.
+Require Import loo_def.
+Require Import chainmail.
+Require Import loo_properties.
+Require Import function_operations.
+Require Import List.
+Require Import CpdtTactics.
+Require Import Coq.Logic.FunctionalExtensionality.
+
+Lemma reduction_preserves_well_formed_heap :
+  forall M σ1 σ2, M ∙ σ1 ⤳ σ2 ->
+             χ_wf M (fst σ1) ->
+             χ_wf M (fst σ2).
+Proof.
+  intros M σ1 σ2 Hred;
+    induction Hred;
+    intros;
+    try solve [crush];
+    subst;
+    apply heap_wf;
+    intros;
+    subst.
+
+  - (*field assign reduce*)
+    simpl in H.
+    unfold update, t_update in H.
+    destruct (eq_dec α0 α) as [Heq|Hneq];
+      [subst; rewrite eqb_refl in H; auto
+      |apply neq_eqb in Hneq; rewrite Hneq in H;
+       inversion H11; subst; apply (H7 α0); auto].
+    inversion H11; subst.
+    destruct (H7 α o (cname o)) as [CDef Hwf]; auto;
+      destruct Hwf as [Hwf1 Hwf2];
+      destruct Hwf2 as [Hwf2 Hwf3].
+    exists CDef; split;
+      [inversion H; subst; auto
+      |split;
+       [intros
+       |inversion H; subst; auto]].
+    inversion H; subst; simpl.
+    destruct (eq_dec f0 f) as [Heq|Hneq];
+      [destruct f0; subst; rewrite <- beq_nat_refl; exists v; auto
+      |destruct f0, f;
+       assert (Hneq' : n <> n0);
+       [intros Hcontra; subst; crush| apply Nat.eqb_neq in Hneq'; rewrite Hneq'; auto]].
+
+  - (*new object initialization*)
+    simpl in *.
+    unfold update, t_update in H0.
+    destruct (eq_dec α0 α) as [Heq|Hneq];
+      [subst; rewrite eqb_refl in H0
+      |apply neq_eqb in Hneq; rewrite Hneq in H0;
+       inversion H9; subst; apply (H6 α0); auto].
+    exists CDef;
+      split; [inversion H0; subst; auto
+             |split;
+              [intros
+              |inversion H0; subst; auto]].
+    inversion H0; subst; simpl.
+    assert (Hin : fMap f = None -> ~ In f (c_flds CDef));
+      [intros;
+       apply not_in_map_implies_not_in_dom with (m:=fMap); auto
+      |].
+    remember (fMap f) as res.
+    destruct res as [y|];
+      [
+      |contradiction Hin; auto].
+    destruct (H5 f y) as [v];
+      auto.
+    exists v; auto.
+Qed.
+
+Ltac reduce_heap_wf_auto :=
+  match goal with
+  | [Hred : ?M ∙ ?σ1 ⤳ ?σ2 |- χ_wf ?M (fst ?σ2)] =>
+    eapply reduction_preserves_well_formed_heap; eauto
+  end.
+
+Lemma reductions_preserves_heap_wf :
+  forall M1 M2 σ1 σ2, M1 ⦂ M2 ⦿ σ1 ⤳… σ2 ->
+                 forall M, M1 ⋄ M2 ≜ M ->
+                      χ_wf M (fst σ1) ->
+                      χ_wf M (fst σ2).
+Proof.
+  intros M1 M2 σ1 σ2 Hred;
+    induction Hred;
+    intros;
+    auto;
+    link_unique_auto;
+    reduce_heap_wf_auto.
+Qed.
+
+Ltac reduces_heap_wf_auto :=
+  match goal with
+  | [Hred : ?M1 ⦂ ?M2 ⦿ ?σ1 ⤳… ?σ2 |- χ_wf ?M (fst ?σ2)] =>
+    eapply reductions_preserves_heap_wf; eauto
+  end.
+
+Lemma pair_reduction_preserves_heap_wf :
+  forall M1 M2 σ1 σ2, M1 ⦂ M2 ⦿ σ1 ⤳ σ2 ->
+                 forall M, M1 ⋄ M2 ≜ M ->
+                      χ_wf M (fst σ1) ->
+                      χ_wf M (fst σ2).
+Proof.
+  intros M1 M2 σ1 σ2 Hred;
+    induction Hred;
+    intros.
+  link_unique_auto.
+  reduce_heap_wf_auto.
+  reduces_heap_wf_auto.
+Qed.
+
+Ltac pair_reduce_heap_wf_auto :=
+  match goal with
+  | [Hred : ?M1 ⦂ ?M2 ⦿ ?σ1 ⤳ ?σ2 |- χ_wf ?M (fst ?σ2)] =>
+    eapply pair_reduction_preserves_heap_wf; eauto
+  end.
+
+Lemma pair_reductions_preserves_heap_wf :
+  forall M1 M2 σ1 σ2, M1 ⦂ M2 ⦿ σ1 ⤳⋆ σ2 ->
+                 forall M, M1 ⋄ M2 ≜ M ->
+                      χ_wf M (fst σ1) ->
+                      χ_wf M (fst σ2).
+Proof.
+  intros M1 M2 σ1 σ2 Hred;
+    induction Hred;
+    intros;
+    auto;
+    try solve pair_reduce_heap_wf_auto.
+  eapply IHHred; eauto;
+    pair_reduce_heap_wf_auto.
+Qed.
+
+Ltac pair_reduces_heap_wf_auto :=
+  match goal with
+  | [Hred : ?M1 ⦂ ?M2 ⦿ ?σ1 ⤳⋆ ?σ2 |- χ_wf ?M (fst ?σ2)] =>
+    eapply pair_reductions_preserves_heap_wf; eauto
+  end.
+
+Ltac obj_defn_rewrite :=
+  match goal with
+  | [H : M_wf ?M |- context[?M ObjectName]] => rewrite (M_wf_ObjectDefn M H)
+  end.
+
+Lemma initial_heap_wf :
+  forall σ, initial σ ->
+       forall M, M_wf M ->
+            χ_wf M (fst σ).
+Proof.
+  intros σ Hinit;
+    destruct Hinit as [α Hinit];
+    destruct Hinit as [ϕ Hinit];
+    andDestruct;
+    subst;
+    intros.
+  apply heap_wf;
+    intros.
+  simpl in H0; inversion H0; subst.
+  update_auto;
+    [exists ObjectDefn;
+     split; simpl; auto;
+     try solve [obj_defn_rewrite; auto];
+     crush
+    |empty_auto].
+Qed.
+
+Ltac initial_heap_wf_auto :=
+  match goal with
+  | [H : initial ?σ |- χ_wf ?M (fst ?σ)] => eapply initial_heap_wf; eauto
+  end.
+
+Lemma linked_wf :
+  forall M1 M2 M, M1 ⋄ M2 ≜ M ->
+             M_wf M1 ->
+             M_wf M2 ->
+             M_wf M.
+Proof.
+  intros M1 M2 M Hlink Hwf1 Hwf2;
+    inversion Hlink; subst;
+      inversion Hwf1; subst;
+        inversion Hwf2; subst.
+  apply module_wf;
+    auto; intros.
+  unfold extend;
+    destruct (M1 ObjectName); auto.
+  unfold extend in H7.
+  remember (M1 C) as x.
+  destruct x; crush.
+  unfold extend in H7.
+  remember (M1 C) as x.
+  destruct x; crush; eauto.
+Qed.
+
+Ltac linking_wf :=
+  match goal with
+  | [H1 : M_wf ?M1, H2 : M_wf ?M2, Hlink : ?M1 ⋄ ?M2 ≜ ?M |- M_wf ?M] => eapply linked_wf; eauto
+  end.
+
+Lemma arising_heap_wf :
+  forall M1 M2 σ, arising M1 M2 σ ->
+             M_wf M1 ->
+             M_wf M2 ->
+             forall M, M1 ⋄ M2 ≜ M ->
+                  χ_wf M (fst σ).
+Proof.
+  intros.
+  inversion H; subst.
+  pair_reduces_heap_wf_auto.
+  initial_heap_wf_auto.
+  linking_wf.
+Qed.
+
+Lemma reduction_preserves_config_finiteness :
+  forall M σ1 σ2, M ∙ σ1 ⤳ σ2 ->
+             finite_σ σ1 ->
+             finite_σ σ2.
+Proof.
+  intros M σ1 σ2 Hred;
+    induction Hred;
+    intros;
+    subst;
+    finite_auto;
+    simpl in *;
+    intros;
+    auto.
+
+  - destruct H0 as [Ha|Ha];
+      [|destruct Ha as [Ha|Ha]];
+      subst;
+      simpl;
+      [apply fin_update;
+       apply finite_map_composition;
+       auto
+      | |];
+      try solve [crush;
+                 eauto];
+      eauto with loo_db.
+
+  - unfold update_ψ_map, update_ϕ_map in H0;
+      inversion H0;
+      subst;
+      [simpl; apply fin_update|];
+      apply H8; crush.
+
+  - destruct H; [subst; simpl|]; eauto.
+
+  - destruct H0; crush.
+
+  - unfold update_ϕ_contn, update_ϕ_map in H; simpl in H;
+      destruct H; crush.
+
+  - unfold update_ϕ_contn, update_ϕ_map in H; simpl in H;
+      destruct H; crush.
+Qed.
+
+Hint Resolve reduction_preserves_config_finiteness : loo_db.
+
+Lemma reductions_preserves_config_finiteness :
+  forall M1 M2 σ1 σ2, M1 ⦂ M2 ⦿ σ1 ⤳… σ2 ->
+                 finite_σ σ1 ->
+                 finite_σ σ2.
+Proof.
+  intros M1 M2 σ1 σ2 Hred;
+    induction Hred;
+    intros;
+    crush;
+    eauto with loo_db.
+Qed.
+
+Hint Resolve reductions_preserves_config_finiteness : loo_db.
+
+Lemma pair_reduction_preserves_config_finiteness :
+  forall M1 M2 σ1 σ2, M1 ⦂ M2 ⦿ σ1 ⤳ σ2 ->
+                 finite_σ σ1 ->
+                 finite_σ σ2.
+Proof.
+  intros M1 M2 σ1 σ2 Hred;
+    inversion Hred;
+    subst;
+    intros;
+    crush;
+    eauto with loo_db.
+Qed.
+
+Hint Resolve pair_reduction_preserves_config_finiteness : loo_db.
+
+Lemma pair_reductions_preserves_config_finiteness :
+  forall M1 M2 σ1 σ2, M1 ⦂ M2 ⦿ σ1 ⤳⋆ σ2 ->
+                 finite_σ σ1 ->
+                 finite_σ σ2.
+Proof.
+  intros M1 M2 σ1 σ2 Hred;
+    induction Hred;
+    subst;
+    intros;
+    eauto with loo_db.
+Qed.
+
+Hint Resolve pair_reductions_preserves_config_finiteness : loo_db.
+
+Lemma reduction_preserves_config_not_stuck :
+  forall M σ1 σ2, M ∙ σ1 ⤳ σ2 ->
+             not_stuck_σ σ1 ->
+             not_stuck_σ σ2.
+Proof.
+  intros M σ1 σ2 Hred;
+    induction Hred;
+    intros;
+    unfold not_stuck_σ in *;
+    simpl in *;
+    try solve [eexists; crush; eauto].
+
+  - exists ϕ'', (ϕ'::ψ); split;
+      unfold not_stuck_ϕ;
+      subst;
+      simpl in *;
+      eauto with loo_db.
+
+  - exists ϕ', ψ;
+      subst;
+      simpl in *;
+      split;
+      auto;
+      unfold not_stuck_ϕ;
+      simpl in *;
+      auto with loo_db.
+
+  - subst σ'; simpl;
+      exists ϕ', ψ;
+      split;
+      auto;
+      subst ϕ';
+      unfold not_stuck_ϕ;
+      simpl;
+      auto with loo_db.
+
+  - exists ϕ', ψ;
+      split;
+      auto;
+      subst;
+      unfold not_stuck_ϕ;
+      simpl;
+      auto with loo_db;
+      crush.
+
+  - exists ϕ'', ψ;
+      split;
+      auto;
+      subst ϕ'';
+      unfold not_stuck_ϕ;
+      simpl;
+      auto with loo_db.
+
+  - exists ϕ'', ψ;
+      split;
+      auto;
+      subst ϕ'';
+      unfold not_stuck_ϕ;
+      simpl;
+      auto with loo_db.
+Qed.
+
+Hint Resolve reduction_preserves_config_not_stuck : loo_db.
+
+Lemma reductions_preserves_config_not_stuck :
+  forall M1 M2 σ1 σ2, M1 ⦂ M2 ⦿ σ1 ⤳… σ2 ->
+                 not_stuck_σ σ1 ->
+                 not_stuck_σ σ2.
+Proof.
+  intros M1 M2 σ1 σ2 Hred;
+    induction Hred;
+    intros;
+    eauto with loo_db.
+Qed.
+
+Hint Resolve reductions_preserves_config_not_stuck : loo_db.
+
+Lemma pair_reduction_preserves_config_not_stuck :
+  forall M1 M2 σ1 σ2, M1 ⦂ M2 ⦿ σ1 ⤳ σ2 ->
+                 not_stuck_σ σ1 ->
+                 not_stuck_σ σ2.
+Proof.
+  intros M1 M2 σ1 σ2 Hred;
+    induction Hred;
+    intros;
+    eauto with loo_db.
+Qed.
+
+Hint Resolve pair_reduction_preserves_config_not_stuck : loo_db.
+
+Lemma pair_reductions_preserves_config_not_stuck :
+  forall M1 M2 σ1 σ2, M1 ⦂ M2 ⦿ σ1 ⤳⋆ σ2 ->
+                 not_stuck_σ σ1 ->
+                 not_stuck_σ σ2.
+Proof.
+  intros M1 M2 σ1 σ2 Hred;
+    induction Hred;
+    intros;
+    eauto with loo_db.
+Qed.
+
+Hint Resolve pair_reductions_preserves_config_not_stuck : loo_db.
+
+Lemma reduction_preserves_config_waiting :
+  forall M σ1 σ2, M ∙ σ1 ⤳ σ2 ->
+             waiting_σ σ1 ->
+             waiting_σ σ2.
+Proof.
+  intros M σ1 σ2 Hred;
+    induction Hred;
+    intros;
+    unfold waiting_σ in *;
+    simpl in *;
+    try solve [eexists; crush; eauto].
+
+  - exists ϕ'', (ϕ'::ψ); split;
+      unfold waiting_ψ, waiting_ϕ in *;
+      subst;
+      intros;
+      auto;
+      match goal with
+      | [H : In ?ϕ0 _ |- waiting (contn ?ϕ0)] => destruct H; subst; crush
+      end.
+
+  - exists ϕ'', ψ; subst;
+      split;
+      auto;
+      unfold waiting_ψ, waiting_ϕ in *;
+      intros;
+      simpl in *;
+      auto;
+      crush.
+
+  - exists ϕ'', ψ; subst;
+      split;
+      auto;
+      unfold waiting_ψ, waiting_ϕ in *;
+      intros;
+      simpl;
+      auto;
+      crush.
+
+Qed.
+
+Hint Resolve reduction_preserves_config_waiting : loo_db.
+
+Lemma reductions_preserves_config_waiting :
+  forall M1 M2 σ1 σ2, M1 ⦂ M2 ⦿ σ1 ⤳… σ2 ->
+                 waiting_σ σ1 ->
+                 waiting_σ σ2.
+Proof.
+  intros M1 M2 σ1 σ2 Hred;
+    induction Hred;
+    intros;
+    eauto with loo_db.
+Qed.
+
+Hint Resolve reductions_preserves_config_waiting : loo_db.
+
+Lemma pair_reduction_preserves_config_waiting :
+  forall M1 M2 σ1 σ2, M1 ⦂ M2 ⦿ σ1 ⤳ σ2 ->
+                 waiting_σ σ1 ->
+                 waiting_σ σ2.
+Proof.
+  intros M1 M2 σ1 σ2 Hred;
+    induction Hred;
+    intros;
+    eauto with loo_db.
+Qed.
+
+Hint Resolve pair_reduction_preserves_config_waiting : loo_db.
+
+Lemma pair_reductions_preserves_config_waiting :
+  forall M1 M2 σ1 σ2, M1 ⦂ M2 ⦿ σ1 ⤳⋆ σ2 ->
+                 waiting_σ σ1 ->
+                 waiting_σ σ2.
+Proof.
+  intros M1 M2 σ1 σ2 Hred;
+    induction Hred;
+    intros;
+    eauto with loo_db.
+Qed.
+
+Hint Resolve pair_reductions_preserves_config_waiting : loo_db.
+
+Lemma reduction_preserves_config_has_self :
+  forall M σ1 σ2, M ∙ σ1 ⤳ σ2 ->
+             has_self_σ σ1 ->
+             has_self_σ σ2.
+Proof.
+  intros M σ1 σ2 Hred;
+    induction Hred;
+    intros Hself;
+    inversion Hself;
+    subst;
+    eauto.
+
+  - (* meth *)
+    inversion H10; subst.
+    apply self_config;
+      intros ϕ' Hin;
+      inversion Hin;
+      auto;
+      [subst|].
+    apply self_frm;
+      exists α, o;
+      split;
+      auto.
+    inversion H0;
+      subst.
+    assert (Hinϕ : In ϕ (ϕ::ψ));
+      [apply in_eq|apply H9 in Hinϕ].
+    apply self_frm;
+      inversion Hinϕ;
+      auto.
+    apply H9;
+      simpl in *;
+      inversion H1;
+      auto.
+
+  - (* var asgn *)
+    apply has_self_update_σ_contn
+      with
+        (c:=c_stmt s)
+      in Hself.
+    apply has_self_update_σ
+      with
+        (x:=x)(v:=v)
+      in Hself;
+      auto.
+
+  - (* field asgn*)
+    inversion H12;
+      subst.
+    apply self_config;
+      intros.
+    inversion H;
+      subst;
+      remember {| cname := cname o; flds := update f v (flds o); meths := meths o |} as o'.
+    assert (Hin : In ϕ (ϕ::ψ));
+      [apply in_eq|apply H11 in Hin].
+    destruct Hin.
+    destruct H7 as [α0 Ha];
+      destruct Ha as [o0];
+      andDestruct.
+    apply self_frm.
+    exists α0.
+    destruct (eq_dec α0 α) as [|Hneq];
+      [subst α0;
+       exists o'
+      |simpl;
+       exists o0];
+      split;
+      simpl;
+      auto;
+      unfold update, t_update;
+      [rewrite eqb_refl; auto
+      |rewrite neq_eqb; auto].  
+    assert (Hin : In ϕ0 (ϕ::ψ));
+      [apply in_cons; auto|apply H11 in Hin].
+    destruct Hin.
+    destruct H8 as [α0 Ha];
+      destruct Ha as [o0];
+      andDestruct.
+    apply self_frm.
+    exists α0.
+    destruct (eq_dec α0 α) as [|Hneq];
+      [subst α0;
+       exists o'
+      |simpl;
+       exists o0];
+      split;
+      simpl;
+      auto;
+      unfold update, t_update;
+      [rewrite eqb_refl; auto
+      |rewrite neq_eqb; auto].
+
+  - (* new *)
+    inversion H10;
+      subst.
+    apply self_config;
+      intros.
+    inversion H0;
+      subst;
+      remember {| cname := C; flds := fMap ∘ (vMap ϕ); meths := c_meths CDef |} as o'.
+    + apply self_frm; simpl.
+      assert (Hin : In ϕ (ϕ::ψ));
+        [apply in_eq
+        |apply H9 in Hin].
+      destruct Hin as [χ ϕ Ha];
+        destruct Ha as [α0 Ha];
+        destruct Ha as [o0];
+        andDestruct.
+      exists α0.
+      destruct (eq_dec α0 α) as [|Hneq];
+        [subst α0;
+         exists o'
+        |simpl;
+         exists o0];
+        simpl;
+        auto;
+        unfold update, t_update;
+        [rewrite neq_eqb; auto
+        |rewrite neq_eqb; auto];
+        split;
+        auto;
+        [rewrite eqb_refl
+        |rewrite neq_eqb; auto];
+        auto.
+
+    + apply self_frm.
+      unfold update, t_update.
+      assert (Hin : In ϕ0 (ϕ::ψ));
+        [apply in_cons; auto
+        |apply H9 in Hin;
+         destruct Hin as [χ ϕ' Ha];
+         destruct Ha as [α0 Ha];
+         destruct Ha as [o0];
+         andDestruct].
+      exists α0.
+      destruct (eq_dec α0 α) as [|Hneq];
+        [subst α0;
+         exists o'
+        |exists o0];
+        [rewrite eqb_refl; auto
+        |rewrite neq_eqb; auto];
+        auto.
+
+  - (* ret 1 *)
+    apply self_config;
+      intros.
+    inversion H6;
+      subst.
+    inversion H;
+      subst.
+    apply has_self_update_ϕ_contn, has_self_update_ϕ;
+      auto.
+    apply H5, in_cons, in_eq.
+    apply H5, in_cons, in_cons;
+      auto.
+
+  - (* ret 2*)
+    apply self_config;
+      intros.
+    inversion H6;
+      subst.
+    inversion H;
+      subst.
+    apply has_self_update_ϕ_contn, has_self_update_ϕ;
+      auto.
+    apply H5.
+    apply in_cons, in_eq.
+    apply H5, in_cons, in_cons;
+      auto.
+Qed.
+
+Hint Resolve reduction_preserves_config_has_self : loo_db.
+
+Lemma reductions_preserves_config_has_self :
+  forall M1 M2 σ1 σ2, M1 ⦂ M2 ⦿ σ1 ⤳… σ2 ->
+                 has_self_σ σ1 ->
+                 has_self_σ σ2.
+Proof.
+  intros M1 M2 σ1 σ2 Hred;
+    induction Hred;
+    intros;
+    eauto with loo_db.
+Qed.
+
+Hint Resolve reduction_preserves_config_has_self : loo_db.
+
+Lemma pair_reduction_preserves_config_has_self :
+  forall M1 M2 σ1 σ2, M1 ⦂ M2 ⦿ σ1 ⤳ σ2 ->
+                 has_self_σ σ1 ->
+                 has_self_σ σ2.
+Proof.
+  intros M1 M2 σ1 σ2 Hred;
+    induction Hred;
+    intros;
+    eauto.
+  eapply reduction_preserves_config_has_self;
+    eauto.
+  eapply reductions_preserves_config_has_self;
+    eauto.
+Qed.
+
+Hint Resolve pair_reduction_preserves_config_has_self : loo_db.
+
+Lemma pair_reductions_preserves_config_has_self :
+  forall M1 M2 σ1 σ2, M1 ⦂ M2 ⦿ σ1 ⤳⋆ σ2 ->
+                 has_self_σ σ1 ->
+                 has_self_σ σ2.
+Proof.
+  intros M1 M2 σ1 σ2 Hred;
+    induction Hred;
+    intros;
+    eauto with loo_db.
+Qed.
+
+Hint Resolve pair_reductions_preserves_config_has_self : loo_db.
+
+Lemma reduction_preserves_config_wf :
+  forall M σ1 σ2, M ∙ σ1 ⤳ σ2 ->
+             σ_wf σ1 ->
+             σ_wf σ2.
+Proof.
+  intros M σ1 σ2 Hred Hwf;
+    inversion Hred;
+    subst;
+    apply config_wf;
+    inversion Hwf;
+    eauto with loo_db;
+    subst.
+Qed.
+
+Hint Resolve reduction_preserves_config_wf : loo_db.
+
+Lemma reductions_preserves_config_wf :
+  forall M1 M2 σ1 σ2, M1 ⦂ M2 ⦿ σ1 ⤳… σ2 ->
+             σ_wf σ1 ->
+             σ_wf σ2.
+Proof.
+  intros M1 M2 σ1 σ2 Hred;
+    induction Hred;
+    intros;
+    subst;
+    eauto with loo_db.
+Qed.
+
+Hint Resolve reductions_preserves_config_wf : loo_db.
+
+Lemma pair_reduction_preserves_config_wf :
+  forall M1 M2 σ1 σ2, M1 ⦂ M2 ⦿ σ1 ⤳ σ2 ->
+                 σ_wf σ1 ->
+                 σ_wf σ2.
+Proof.
+  intros M1 M2 σ1 σ2 Hred Hwf;
+    induction Hred;
+    eauto with loo_db.
+Qed.
+
+Hint Resolve pair_reduction_preserves_config_wf : loo_db.
+
+Lemma pair_reductions_preserves_config_wf :
+  forall M1 M2 σ1 σ2, M1 ⦂ M2 ⦿ σ1 ⤳⋆ σ2 ->
+                 σ_wf σ1 ->
+                 σ_wf σ2.
+Proof.
+  intros M1 M2 σ1 σ2 Hred Hwf;
+    induction Hred;
+    eauto with loo_db.
+Qed.
+
+Hint Resolve pair_reductions_preserves_config_wf : loo_db.
+
+Lemma arising_wf :
+  forall M1 M2 σ, arising M1 M2 σ ->
+             σ_wf σ.
+Proof.
+  intros M1 M2 σ Harise.
+  inversion Harise;
+    subst.
+  eapply pair_reductions_preserves_config_wf; eauto with loo_db.
+Qed.
+
+Hint Resolve arising_wf : loo_db.
+
+Theorem eval_unique :
+  forall M σ e v1, M ∙ σ ⊢ e ↪ v1 ->
+              forall v2, M ∙ σ ⊢ e ↪ v2 ->
+                    v2 = v1.
+Proof.
+  intros M σ e v1 Heval;
+    induction Heval;
+    intros;
+    try solve [inversion H; subst; [eauto| eauto];
+               apply IHHeval1 in H6; inversion H6].
+
+  (** Case 1: eval v *)
+  inversion H; eauto.
+
+  (** Case 2: eval x *)
+  inversion H0; subst; crush.
+
+  (** Case 3: e.f *)
+  inversion H1; subst; crush.
+  apply IHHeval in H4; subst; crush.
+
+  (** Case 4: e0.g(e) *)
+  inversion H2; subst.
+  apply IHHeval1 in H6; inversion H6; subst.
+  rewrite H7 in H; inversion H; subst.
+  rewrite H8 in H0; inversion H0; subst.
+  rewrite H11 in H1; inversion H1; subst.
+  apply IHHeval2 in H13; subst.
+  apply IHHeval3 in H14; subst; auto.
+
+  (** Case 5: e1 = e2 *) 
+  inversion H; subst; eauto.
+  apply IHHeval1 in H2; apply IHHeval2 in H5; subst; crush.
+
+  (** Case 6: e1 ≠ e2 *)
+  inversion H0; subst; eauto.
+  apply IHHeval1 in H5; apply IHHeval2 in H7; subst; crush.
+Qed.
+
+Hint Rewrite eval_unique : loo_db.
+
+Ltac eval_rewrite :=
+  repeat match goal with
+         | [H1 : ?M ∙ ?σ ⊢ ?e ↪ ?v1, H2 : ?M ∙ ?σ ⊢ ?e ↪ ?v2 |- _] =>
+           eapply (eval_unique M σ e v1 H1) in H2;
+           eauto;
+           subst
+         end.
+
+Lemma pair_reductions_transitive :
+  forall M1 M2 σ1 σ2, M1 ⦂ M2 ⦿ σ1 ⤳⋆ σ2 ->
+                 forall σ3, M1 ⦂ M2 ⦿ σ2 ⤳⋆ σ3 ->
+                       M1 ⦂ M2 ⦿ σ1 ⤳⋆ σ3.
+Proof.
+  intros M1 M2 σ1 σ2 Hred;
+    induction Hred;
+    intros;
+    eauto with loo_db.
+Qed.
+
+Lemma reduction_preserves_addr_classes :
+  forall M σ1 σ2, M ∙ σ1 ⤳ σ2 ->
+             forall (α : addr) o1,
+               mapp σ1 α = Some o1 ->
+               exists o2, mapp σ2 α = Some o2 /\
+                     cname o2 = cname o1.
+Proof.
+  intros M σ1 σ2 Hred;
+    destruct Hred;
+    intros;
+    subst;
+    eauto;
+    unfold mapp, configMapHeap in *;
+    simpl in *.
+
+  - (* asgn fld*)
+    destruct (eq_dec α0 α) as [|Hneq];
+      [subst|].
+    + exists {| cname := cname o; flds := update f v (flds o); meths := meths o |};
+        simpl;
+        unfold update, t_update;
+        rewrite eqb_refl;
+        split;
+        simpl;
+        crush.
+
+    + exists o1;
+        unfold update, t_update;
+        rewrite neq_eqb;
+        auto.
+
+  - destruct (eq_dec α0 α) as [|Hneq];
+      [subst; eapply fresh_heap_some_contradiction; eauto|].
+
+    + exists o1;
+        unfold update, t_update;
+        rewrite neq_eqb;
+        auto.
+  
+Qed.
+
+Hint Resolve reduction_preserves_addr_classes : loo_db.
+Hint Rewrite reduction_preserves_addr_classes : loo_db.
+
+Lemma reductions_preserves_addr_classes :
+  forall M1 M2 σ1 σ2, M1 ⦂ M2 ⦿ σ1 ⤳… σ2 ->
+                 forall (α : addr) o1,
+                   mapp σ1 α = Some o1 ->
+                   exists o2, mapp σ2 α = Some o2 /\
+                   cname o2 = cname o1.
+Proof.
+  intros M1 M2 σ1 σ2 Hred;
+    induction Hred;
+    intros;
+    eauto with loo_db.
+
+  destruct IHHred with (α:=α)(o1:=o1) as [o Hclass];
+    eauto; auto;
+      andDestruct.
+
+  edestruct reduction_preserves_addr_classes as [o' Hclass1];
+    eauto.
+
+  andDestruct.
+
+  eexists; split; eauto; crush.
+Qed.
+
+Hint Resolve reductions_preserves_addr_classes : loo_db.
+Hint Rewrite reductions_preserves_addr_classes : loo_db.
+
+Lemma pair_reduction_preserves_addr_classes :
+  forall M1 M2 σ1 σ2, M1 ⦂ M2 ⦿ σ1 ⤳ σ2 ->
+                 forall (α : addr) o1,
+                   mapp σ1 α = Some o1 ->
+                   exists o2, mapp σ2 α = Some o2 /\
+                         cname o2 = cname o1.
+Proof.
+  intros M1 M2 σ1 σ2 Hred;
+    induction Hred;
+    intros;
+    eauto with loo_db.
+Qed.
+
+Hint Resolve pair_reduction_preserves_addr_classes : loo_db.
+Hint Rewrite pair_reduction_preserves_addr_classes : loo_db.
+
+Lemma pair_reductions_preserves_addr_classes :
+  forall M1 M2 σ1 σ2, M1 ⦂ M2 ⦿ σ1 ⤳⋆ σ2 ->
+                 forall (α : addr) o1,
+                   mapp σ1 α = Some o1 ->
+                   exists o2, mapp σ2 α = Some o2 /\
+                         cname o2 = cname o1.
+Proof.
+  intros M1 M2 σ1 σ2 Hred;
+    induction Hred;
+    intros;
+    eauto with loo_db.
+
+  destruct (pair_reduction_preserves_addr_classes M1 M2 σ1 σ)
+    with
+      (α:=α)(o1:=o1)
+    as [o Hclass1];
+    auto;
+    andDestruct.
+
+  edestruct IHHred as [o' Hclass2];
+    eauto;
+    andDestruct.
+
+  eexists; split; eauto; crush.
+  
+Qed.
+
+Hint Resolve pair_reductions_preserves_addr_classes : loo_db.
+Hint Rewrite pair_reductions_preserves_addr_classes : loo_db.
+
+Lemma reduction_unique :
+  forall M σ σ1, M ∙ σ ⤳ σ1 ->
+            forall σ2, M ∙ σ ⤳ σ2 ->
+                  σ2 = σ1.
+Proof.
+  intros M σ σ1 Hred;
+    induction Hred;
+    intros.
+
+  - (* meth *)
+    simpl in *;
+      subst.
+    inversion H2;
+      subst;
+      crush.
+    inversion H9;
+      subst;
+      crush.
+    inversion H8; subst.
+    rewrite H1 in H10.
+    inversion H10; subst.
+    interpretation_rewrite.
+    crush.
+
+  - (* vAssgn *)
+    inversion H8;
+      subst;
+      crush.
+    inversion H10; subst.
+    rewrite H1 in H11;
+      inversion H11;
+      subst.
+    interpretation_rewrite;
+      crush.
+
+  - (* fAssgn *)
+    simpl in *.
+    inversion H11;
+      subst;
+      crush.
+    inversion H12; subst.
+    rewrite H13 in H0;
+      inversion H0;
+      subst.
+    interpretation_rewrite.
+    crush.
+
+  - (* new *)
+    inversion H9;
+      subst;
+      crush.
+    inversion H11; subst.
+    rewrite H1 in H12;
+      inversion H12;
+      subst;
+      crush.
+    match goal with
+    | [H1 : fresh_χ ?χ ?αa,
+            H2 : fresh_χ ?χ ?αb |- _] =>
+      apply fresh_heap_unique with (α1:=αa) in H2;
+        subst;
+        auto
+    end.
+    crush.
+
+  - (* ret1 *)
+    subst.
+    inversion H5;
+      subst;
+      crush.
+    inversion H; subst.
+    rewrite H0 in H4;
+      inversion H4;
+      subst.
+    interpretation_rewrite.
+    crush.
+
+
+  - crush.
+    inversion H5;
+      subst;
+      crush.
+    inversion H;
+      subst.
+    rewrite H0 in H4;
+      inversion H4;
+      subst.
+    interpretation_rewrite.
+    crush.
+
+Qed.
+
+Hint Resolve reduction_unique : loo_db.
+
+Lemma pair_reduction_unique :
+  forall M1 M2 σ σ1, M1 ⦂ M2 ⦿ σ ⤳ σ1 ->
+                forall σ2, M1 ⦂ M2 ⦿ σ ⤳ σ2 ->
+                      σ1 = σ2.
+Proof.
+Admitted.
